@prefix p4-lucat: <http://p4-lucat.eu/vocab/> .
@prefix owl: <http://www.w3.org/2002/07/owl#> .
@prefix rdf: <http://www.w3.org/1999/02/22-rdf-syntax-ns#> .
@prefix rdfs: <http://www.w3.org/2000/01/rdf-schema#> .
@prefix xsd: <http://www.w3.org/2001/XMLSchema#> .
@prefix dcterms: <http://purl.org/dc/terms/> .
@prefix prv: <http://purl.org/net/provenance/ns#> .

##########################################################################################
################################## Classes ###############################################
##########################################################################################
p4-lucat:Assignment 		rdf:type 	owl:Class;
                                      		rdfs:subClassOf p4-lucat:Concept;
                                      		rdfs:comment "This class represents the assignment of a clinical trial"@en;
                                      		rdfs:isDefinedBy "emetis_niazmand"@en;
						rdfs:label "Assignment"@en;
						owl:versionInfo "v1.0"@en.

p4-lucat:Assignment-Annotation 	rdf:type 	owl:Class ;
						rdfs:subClassOf p4-lucat:Concept;
						rdfs:comment "This class represents the assignment-Annotation of a clinical trial"@en;
						rdfs:isDefinedBy "emetis_niazmand"@en;
						rdfs:label "hasAssignment"@en;
						owl:versionInfo "v1.0"@en.

p4-lucat:Gender		 	rdf:type 	owl:Class;
						rdfs:subClassOf p4-lucat:Concept;
						rdfs:comment "This class represents the gender included in a clinical trial"@en;
						rdfs:isDefinedBy "emetis_niazmand"@en;
						rdfs:label "Sex"@en;
						owl:versionInfo "v1.0"@en.



p4-lucat:ClinicalTrial 		rdf:type 	owl:Class;
						rdfs:subClassOf p4-lucat:Concept;
						rdfs:comment "This class represents clinical trials conducted to study lung cancer drugs"@en;
						rdfs:isDefinedBy "emetis_niazmand"@en;
						rdfs:label "ClinicalTrial"@en;
						owl:versionInfo "v1.0"@en.


p4-lucat:Concept 		rdf:type 	owl:Class;
						rdfs:subClassOf owl:Thing;
						rdfs:comment "Constituents of thoughts or real world entities."@en;
						rdfs:isDefinedBy "emetis_niazmand"@en;
						rdfs:label "Concept"@en;
						owl:versionInfo "v1.0"@en.

p4-lucat:Condition-Annotation 	rdf:type 	owl:Class ;
						rdfs:subClassOf p4-lucat:Concept;
						rdfs:comment "This class represents condition-Annotation"@en;
						rdfs:isDefinedBy "emetis_niazmand"@en;
						rdfs:label "annConditionLabel"@en;
						owl:versionInfo "v1.0"@en.

p4-lucat:Condition 		rdf:type 	owl:Class;
						rdfs:subClassOf p4-lucat:Disorder;
						rdfs:comment "This class represents conditions or diseases"@en;
						rdfs:isDefinedBy "emetis_niazmand"@en;
						rdfs:label "hasCondition"@en;
						owl:versionInfo "v1.0"@en.


p4-lucat:Disorder 		rdf:type 	owl:Class;
						rdfs:subClassOf p4-lucat:Concept;
						rdfs:comment "This class represents disorders"@en;
						rdfs:isDefinedBy "emetis_niazmand"@en;
						rdfs:label "Disorder"@en;
						owl:versionInfo "v1.0"@en.


p4-lucat:Drug 			rdf:type 	owl:Class;
						rdfs:subClassOf p4-lucat:Intervention;
						rdfs:comment "This class represents drugs"@en;
						rdfs:isDefinedBy "emetis_niazmand"@en;
						rdfs:label "Drug"@en;
						owl:versionInfo "v1.0"@en.

p4-lucat:Intervention-Annotation 	rdf:type 	owl:Class ;
							rdfs:subClassOf p4-lucat:Concept;
							rdfs:comment "This class represents intervention-Annotation of clinical trials (e.g., drugs, medical devices)"@en;
							rdfs:isDefinedBy "emetis_niazmand"@en;
							rdfs:label "annInterventionLabel"@en;
							owl:versionInfo "v1.0"@en.

p4-lucat:Intervention 		rdf:type 	owl:Class;
						rdfs:subClassOf p4-lucat:Concept;
						rdfs:comment "This class represents interventions of clinical trials (e.g., drugs, medical devices)"@en;
						rdfs:isDefinedBy "emetis_niazmand"@en;
						rdfs:label "hasIntervention"@en;
						owl:versionInfo "v1.0"@en.


p4-lucat:Keyword-Annotation 	rdf:type 	owl:Class ;
						rdfs:subClassOf p4-lucat:Concept;
						rdfs:comment "This class represents medical Keyword-Annotation"@en;
						rdfs:isDefinedBy "emetis_niazmand"@en;
						rdfs:label "annKeywordLabel"@en;
						owl:versionInfo "v1.0"@en.


p4-lucat:Keyword 		rdf:type 	owl:Class ;
						rdfs:subClassOf p4-lucat:Concept;
						rdfs:comment "This class represents medical keywords"@en;
						rdfs:isDefinedBy "emetis_niazmand"@en;
						rdfs:label "hasKeyword"@en;
						owl:versionInfo "v1.0"@en.

p4-lucat:NLPTool		rdf:type 	owl:Class ;
						rdfs:subClassOf p4-lucat:Concept;
						rdfs:comment "This class represents NLP tools SciSpacy and BioFALCON"@en;
						rdfs:isDefinedBy "emetis_niazmand"@en;
						rdfs:label "sourceName"@en;
						owl:versionInfo "v1.0"@en.

p4-lucat:Stages			rdf:type 	owl:Class ;
						rdfs:subClassOf p4-lucat:Concept;
						rdfs:comment "This class represents Stages"@en;
						rdfs:isDefinedBy "emetis_niazmand"@en;
						rdfs:label "Stages"@en;
						owl:versionInfo "v1.0"@en.

p4-lucat:Publication 		rdf:type 	owl:Class;
						rdfs:subClassOf p4-lucat:Concept;
						rdfs:comment "This class represents scientific publications"@en;
						rdfs:isDefinedBy "emetis_niazmand"@en;
						rdfs:label "Publication"@en;
						owl:versionInfo "v1.0"@en.


p4-lucat:Annotation		rdf:type	owl:Class;
						rdfs:label	"Annotation";
						rdfs:comment "Explanation of a concept including label, id and source of concept.";
						dcterms:description "e.g. CUI IDs provided by UMLS.";
						dcterms:modified "2017-10-23"^^xsd:date;
						dcterms:creator <https://www.tib.eu/en/research-development/scientific-data-management/staff/maria-esther-vidal>.

p4-lucat:Relation		rdf:type	owl:Class;
						rdfs:label	"Relation";
						rdfs:comment "Relations between concepts.";
						dcterms:modified "2017-10-23"^^xsd:date;
						dcterms:creator <https://www.tib.eu/en/research-development/scientific-data-management/staff/maria-esther-vidal>.

p4-lucat:SourceName		rdf:type	owl:Class;
						rdfs:label	"SourceName";
						rdfs:comment "Source name.";
						dcterms:modified "2017-10-23"^^xsd:date;
						dcterms:creator <https://www.tib.eu/en/research-development/scientific-data-management/staff/samaneh-jozashoori/>.

p4-lucat:Image 			rdf:type 	owl:Class;
						rdfs:label	"MedicalImage";
						rdfs:subClassOf	p4-lucat:Concept;
						p4-lucat:partOf p4-lucat:ClinicalRecord;
						rdfs:comment "Patient's medical images.";
						dcterms:modified "2017-10-23"^^xsd:date;
						dcterms:creator <https://www.tib.eu/en/research-development/scientific-data-management/staff/maria-esther-vidal>.

p4-lucat:Test 			rdf:type 	owl:Class;
						rdfs:label	"MedicalTest";
						rdfs:subClassOf	p4-lucat:Concept;
						p4-lucat:partOf p4-lucat:ClinicalRecord;
						rdfs:comment "Medical procedure performed to detect, diagnose, or monitor diseases, disease processes, susceptibility, and determine a course of treatment.";
						dcterms:modified "2017-10-23"^^xsd:date;
						dcterms:creator <https://www.tib.eu/en/research-development/scientific-data-management/staff/maria-esther-vidal>.

p4-lucat:Interaction		rdf:type 	owl:Class;
						rdfs:label	"Interaction";
						rdfs:subClassOf	p4-lucat:Concept;
						rdfs:comment "Interaction between drugs and disorder, enzyme, target.";
						dcterms:modified "2020-07-24"^^xsd:date;
						dcterms:creator <https://www.tib.eu/en/research-development/scientific-data-management/staff/samaneh-jozashoori/>.			

#### WP4 requirements: 

p4-lucat:Author			rdf:type	owl:Class;
						rdfs:label	"Author";
						rdfs:subClassOf	p4-lucat:Concept;
						rdfs:comment "Author of Scientific publications.";
						dcterms:modified "2019-05-24"^^xsd:date;
						dcterms:creator <https://www.tib.eu/en/research-development/scientific-data-management/staff/maria-isabel-castellanos/>.

p4-lucat:MENTIONED_IN		rdf:type 	owl:Class;
						rdfs:label	"MentionedIn";
						rdfs:subClassOf p4-lucat:Relation;
						rdfs:comment	"A relation that shows in which publication each specific CUI term has been appeared.";
						dcterms:modified "2017-10-23"^^xsd:date;
						dcterms:creator <https://www.tib.eu/en/research-development/scientific-data-management/staff/maria-esther-vidal>.

p4-lucat:HAS_TOPIC		rdf:type 	owl:Class;
						rdfs:label	"HasTopic";
						rdfs:subClassOf p4-lucat:Relation;
						rdfs:comment	"A relation that shows which CUI has been appeared in each specific publication.";
						dcterms:modified "2017-10-23"^^xsd:date;
						dcterms:creator <https://www.tib.eu/en/research-development/scientific-data-management/staff/samaneh-jozashoori/>.

p4-lucat:ASSOCIATED_WITH	rdf:type 	owl:Class;
						rdfs:label	"AssociatedWith";
						rdfs:subClassOf p4-lucat:Relation;
						rdfs:comment	"UMLS Annotation.";
						dcterms:modified "2017-10-23"^^xsd:date;
						dcterms:creator <https://www.tib.eu/en/research-development/scientific-data-management/staff/maria-esther-vidal>.

p4-lucat:CAUSES			rdf:type 	owl:Class;
						rdfs:label	"Causes";
						rdfs:subClassOf p4-lucat:Relation;
						rdfs:comment	"UMLS Annotation.";
						dcterms:modified "2017-10-23"^^xsd:date;
						dcterms:creator <https://www.tib.eu/en/research-development/scientific-data-management/staff/samaneh-jozashoori/>.

p4-lucat:INHIBITS		rdf:type 	owl:Class;
						rdfs:label	"Inhibits";
						rdfs:subClassOf p4-lucat:Relation;
						rdfs:comment	"UMLS Annotation.";
						dcterms:modified "2017-10-23"^^xsd:date;
						dcterms:creator <https://www.tib.eu/en/research-development/scientific-data-management/staff/samaneh-jozashoori/>.

p4-lucat:INTERACTS_WITH 	rdf:type 	owl:Class;
						rdfs:label	"InteractsWith";
						rdfs:subClassOf p4-lucat:Relation;
						rdfs:comment	"UMLS Annotation.";
						dcterms:modified "2017-10-23"^^xsd:date;
						dcterms:creator <https://www.tib.eu/en/research-development/scientific-data-management/staff/samaneh-jozashoori/>.

p4-lucat:PREDISPOSES 		rdf:type 	owl:Class;
						rdfs:label	"Predisposes";
						rdfs:subClassOf p4-lucat:Relation;
						rdfs:comment	"UMLS Annotation.";
						dcterms:modified "2017-10-23"^^xsd:date;
						dcterms:creator <https://www.tib.eu/en/research-development/scientific-data-management/staff/samaneh-jozashoori/>.

p4-lucat:STIMULATES 		rdf:type 	owl:Class;
						rdfs:label	"Stimulates";
						rdfs:subClassOf p4-lucat:Relation;
						rdfs:comment	"UMLS Annotation.";
						dcterms:modified "2017-10-23"^^xsd:date;
						dcterms:creator <https://www.tib.eu/en/research-development/scientific-data-management/staff/samaneh-jozashoori/>.


#### Drug requirements:

p4-lucat:LungCancerDrug		rdf:type 	owl:Class;
						rdfs:label	"LungCancerDrug";
						rdfs:subClassOf	p4-lucat:Drug;
						rdfs:comment "Drugs that are prescibied for lung cancer.";
						dcterms:modified "2020-07-24"^^xsd:date;
						dcterms:creator <https://www.tib.eu/en/research-development/scientific-data-management/staff/samaneh-jozashoori/>.


p4-lucat:Phenotype 		rdf:type	owl:Class;
						rdfs:label	"Phenotype";
						rdfs:subClassOf	p4-lucat:Concept;
						rdfs:comment "The set of observable characteristics of an individual resulting from the interaction of its genotype with the environment. This class include side effects that result from different drugs.";
						dcterms:modified "2019-01-30"^^xsd:date;
						dcterms:creator <https://www.tib.eu/en/research-development/scientific-data-management/staff/samaneh-jozashoori/>.


p4-lucat:DrugSideEffect		rdf:type 	owl:Class;
						rdfs:label	"DrugSideEffect";
						rdfs:subClassOf	p4-lucat:Relation;
						rdfs:comment "The Drug SideEffect relation should be a class since has two properties";
						dcterms:modified "2017-07-24"^^xsd:date;
						dcterms:creator <https://www.tib.eu/en/research-development/scientific-data-management/staff/samaneh-jozashoori/>.

p4-lucat:Enzyme			rdf:type 	owl:Class;
						rdfs:label	"Enzyme";
						rdfs:subClassOf	p4-lucat:Concept;
						rdfs:comment "Macromolecular biological catalyst that accelerate chemical reactions. Most enzymes are proteins.";
						dcterms:modified "2017-07-24"^^xsd:date;
						dcterms:creator <https://www.tib.eu/en/research-development/scientific-data-management/staff/samaneh-jozashoori/>.

p4-lucat:EffectInteraction	rdf:type 	owl:Class;
						rdfs:label	"EffectInteraction";
						rdfs:subClassOf	p4-lucat:Relation;
						rdfs:comment "The relation between two drugs that interact.";
						dcterms:modified "2018-10-23"^^xsd:date;
						dcterms:creator <https://www.tib.eu/en/research-development/scientific-data-management/staff/samaneh-jozashoori/>.


p4-lucat:Target			rdf:type 	owl:Class;
						rdfs:label	"Target";
						rdfs:subClassOf	p4-lucat:Concept;
						rdfs:comment "A drug target is a molecule in the body, usually a protein, that is intrinsically associated with a particular disease process and that could be addressed by a drug to produce a desired therapeutic effect.";
						dcterms:modified "2018-10-30"^^xsd:date;
						dcterms:creator <https://www.tib.eu/en/research-development/scientific-data-management/staff/samaneh-jozashoori/>.

p4-lucat:Protein		rdf:type 	owl:Class;
						rdfs:label	"Protein";
						rdfs:subClassOf	p4-lucat:Concept;
						rdfs:comment "Represents large biomolecules, or macromolecules, consisting of one or more long chains of amino acid residues.";
						dcterms:modified "2020-07-24"^^xsd:date;
						dcterms:creator <https://www.tib.eu/en/research-development/scientific-data-management/staff/samaneh-jozashoori/>.

p4-lucat:PredictedDrugSideEffect	rdf:type 	owl:Class;
							rdfs:label	"PredictedDrugSideEffect";
							rdfs:subClassOf	p4-lucat:Relation;
							rdfs:comment "The predicted Drug SideEffect relation.";
							dcterms:modified "2019-01-30"^^xsd:date;
							dcterms:creator <https://www.tib.eu/en/research-development/scientific-data-management/staff/samaneh-jozashoori/>.	

p4-lucat:DrugDisorderInteraction	rdf:type 	owl:Class;
							rdfs:label	"DrugDisorderInteraction";
							rdfs:subClassOf	p4-lucat:Interaction;
							rdfs:comment "Represents the relation between drugs and disorders.";
							dcterms:modified "2020-07-24"^^xsd:date;
							dcterms:creator <https://www.tib.eu/en/research-development/scientific-data-management/staff/samaneh-jozashoori/>.		

p4-lucat:DrugSideEffectInteraction	rdf:type 	owl:Class;
							rdfs:label	"DrugSideEffectInteraction";
							rdfs:subClassOf	p4-lucat:Interaction;
							rdfs:comment "Represents side effects of drugs.";
							dcterms:modified "2020-07-24"^^xsd:date;
							dcterms:creator <https://www.tib.eu/en/research-development/scientific-data-management/staff/samaneh-jozashoori/>.		

p4-lucat:DrugTargetInteraction		rdf:type 	owl:Class;
							rdfs:label	"DrugTargetInteraction";
							rdfs:subClassOf	p4-lucat:Interaction;
							rdfs:comment "Represents the relation between drugs and targets.";
							dcterms:modified "2020-07-24"^^xsd:date;
							dcterms:creator <https://www.tib.eu/en/research-development/scientific-data-management/staff/samaneh-jozashoori/>.		

p4-lucat:DrugEnzymeInteraction		rdf:type 	owl:Class;
							rdfs:label	"DrugEnzymeInteraction";
							rdfs:subClassOf	p4-lucat:Interaction;
							rdfs:comment "Represents the relation between drugs and enzymes.";
							dcterms:modified "2020-07-24"^^xsd:date;
							dcterms:creator <https://www.tib.eu/en/research-development/scientific-data-management/staff/samaneh-jozashoori/>.		

p4-lucat:DrugDrugInteraction		rdf:type 	owl:Class;
							rdfs:label	"DrugDrugInteraction";
							rdfs:subClassOf	p4-lucat:Interaction;
							rdfs:comment "Represents the relation between drugs.";
							dcterms:modified "2020-07-24"^^xsd:date;
							dcterms:creator <https://www.tib.eu/en/research-development/scientific-data-management/staff/samaneh-jozashoori/>.		

p4-lucat:SymmetricDrugDrugInteraction	rdf:type 	owl:Class;
							rdfs:label	"SymmetricDrugDrugInteraction";
							rdfs:subClassOf	p4-lucat:Interaction;
							rdfs:comment "Represents the symmetric relation between drugs.";
							dcterms:modified "2020-07-24"^^xsd:date;
							dcterms:creator <https://www.tib.eu/en/research-development/scientific-data-management/staff/samaneh-jozashoori/>.	

p4-lucat:AdverseEvent		rdf:type 	owl:Class;
						rdfs:label	"AdverseEvent";
						rdfs:subClassOf	p4-lucat:Concept;
						rdfs:comment "Represents the consequence of the interaction between two drugs.";
						dcterms:modified "2020-07-24"^^xsd:date;
						dcterms:creator <https://www.tib.eu/en/research-development/scientific-data-management/staff/samaneh-jozashoori/>.																																					

p4-lucat:DrugDrugPrediction	rdf:type 	owl:Class;
						rdfs:label	"DrugDrugPrediction";
						rdfs:subClassOf	p4-lucat:Interaction;
						rdfs:comment "Represents the predicted relation between drugs.";
						dcterms:modified "2020-10-29"^^xsd:date;
						dcterms:creator <https://www.tib.eu/en/research-development/scientific-data-management/staff/samaneh-jozashoori/>.

p4-lucat:DrugEnzymePrediction	rdf:type 	owl:Class;
						rdfs:label	"DrugEnzymePrediction";
						rdfs:subClassOf	p4-lucat:Interaction;
						rdfs:comment "Represents the predicted relation between drug and enzyme.";
						dcterms:modified "2020-10-29"^^xsd:date;
						dcterms:creator <https://www.tib.eu/en/research-development/scientific-data-management/staff/samaneh-jozashoori/>.

p4-lucat:DrugSideEffectPrediction	rdf:type 	owl:Class;
							rdfs:label	"DrugSideEffectPrediction";
							rdfs:subClassOf	p4-lucat:Interaction;
							rdfs:comment "Represents the predicted relation between drug and side effects.";
							dcterms:modified "2020-10-29"^^xsd:date;
							dcterms:creator <https://www.tib.eu/en/research-development/scientific-data-management/staff/samaneh-jozashoori/>.

p4-lucat:DrugTargetPrediction		rdf:type 	owl:Class;
							rdfs:label	"DrugTargetPrediction";
							rdfs:subClassOf	p4-lucat:Interaction;
							rdfs:comment "Represents the predicted relation between drug and target.";
							dcterms:modified "2020-10-29"^^xsd:date;
							dcterms:creator <https://www.tib.eu/en/research-development/scientific-data-management/staff/samaneh-jozashoori/>.

p4-lucat:PublicationType	rdf:type 	owl:Class;
						rdfs:label	"PublicationType";
						rdfs:subClassOf	p4-lucat:Concept;
						rdfs:comment "Represents the predicted relation between drug and target.";
						dcterms:modified "2020-10-29"^^xsd:date;
						dcterms:creator <https://www.tib.eu/en/research-development/scientific-data-management/staff/samaneh-jozashoori/>.

#### WP2 requirements:
#### clinical notes:

p4-lucat:Observation    	rdf:type        owl:Class;
						rdfs:label	"p4-lucat:Observation";
						rdfs:subClassOf	 p4-lucat:Concept;
						rdfs:comment "Any record that relates to monitoring a process.";
						dcterms:modified "2018-11-27"^^xsd:date;
						dcterms:creator <https://www.tib.eu/en/research-development/scientific-data-management/staff/samaneh-jozashoori/>.

p4-lucat:Patient 		rdf:type 	owl:Class;
						rdfs:label	"Patient";
						rdfs:subClassOf	p4-lucat:Concept;
						rdfs:comment "A person who is receiving medical care.";
						dcterms:modified "2018-07-24"^^xsd:date;
						dcterms:creator <https://www.tib.eu/en/research-development/scientific-data-management/staff/samaneh-jozashoori/>.

p4-lucat:LCPatient		rdf:type 	owl:Class;
						rdfs:label	"LungCancerPatient";
						rdfs:subClassOf	p4-lucat:Patient;
						rdfs:comment "A patient who is diagnosed with Lung Cancer.";
						dcterms:modified "2018-07-24"^^xsd:date;
						dcterms:creator <https://www.tib.eu/en/research-development/scientific-data-management/staff/samaneh-jozashoori/>.
	
p4-lucat:LiquidBiopsy 		rdf:type 	owl:Class;
						rdfs:label	"LiquidBiopsy";
						rdfs:subClassOf	p4-lucat:Test;
						rdfs:comment	"A test done on a sample of blood to look for cancer cells from a tumor that are circulating in the blood or for pieces of DNA from tumor cells that are in the blood.";
						dcterms:modified "2018-07-24"^^xsd:date;
						dcterms:creator <https://www.tib.eu/en/research-development/scientific-data-management/staff/samaneh-jozashoori/>.

p4-lucat:TumorStage		rdf:type 	owl:Class;
						rdfs:label	"TumorStage";
						rdfs:comment "Represents the assessment of the stage of tumor in a particular date.";
						dcterms:modified "2018-10-04"^^xsd:date;
						dcterms:creator <https://www.tib.eu/en/research-development/scientific-data-management/staff/samaneh-jozashoori/>.

p4-lucat:PerformanceStatus	rdf:type	owl:Class;
						rdfs:label	"PerformanceStatus";
						rdfs:comment "Patient's level of functioning in terms of her/his ability for caring her/himself, daily activities and phyical abilities.";
						dcterms:modified "2018-09-27"^^xsd:date;
						dcterms:creator <https://www.tib.eu/en/research-development/scientific-data-management/staff/samaneh-jozashoori/>.

p4-lucat:FamiliarAntecedent	rdf:type	owl:Class;
						rdfs:label	"FamiliarAntecedent";
						rdfs:comment "Familiar antecedents of the patient.";
						dcterms:modified "2018-09-27"^^xsd:date;
						dcterms:creator <https://www.tib.eu/en/research-development/scientific-data-management/staff/samaneh-jozashoori/>.

p4-lucat:DrugGroup		rdf:type	owl:Class;
						rdfs:subClassOf p4-lucat:Concept;
						rdfs:label	"DrugGroup";
						rdfs:comment "The type of drugs that has been prescribed to the patient.";
						dcterms:modified "2018-10-04"^^xsd:date;
						dcterms:creator <https://www.tib.eu/en/research-development/scientific-data-management/staff/samaneh-jozashoori/>.


p4-lucat:TumorType		rdf:type	owl:Class;
						rdfs:subClassOf p4-lucat:Concept;
						rdfs:label	"TumorType";
						rdfs:comment "The histology kind of the lung cancer. The type of tumor.";
						dcterms:modified "2018-10-04"^^xsd:date;
						dcterms:creator <https://www.tib.eu/en/research-development/scientific-data-management/staff/samaneh-jozashoori/>.

p4-lucat:Biomarker	 	rdf:type	owl:Class;
						rdfs:label	"Biomarker";
						rdfs:subClassOf	p4-lucat:Concept;
						rdfs:comment "A biomarker, or biological marker is a measurable indicator of some biological state or condition.";
						dcterms:modified "2018-11-22"^^xsd:date;
						dcterms:creator <https://www.tib.eu/en/research-development/scientific-data-management/staff/maria-isabel-castellanos/>.

p4-lucat:PerformanceObservation   rdf:type      owl:Class;
						rdfs:label	"p4-lucat:PerformanceObservation";
						rdfs:subClassOf	p4-lucat:Observation;
						rdfs:comment "";
						dcterms:modified "2018-11-27"^^xsd:date;
						dcterms:creator <https://www.tib.eu/en/research-development/scientific-data-management/staff/maria-isabel-castellanos/>.

p4-lucat:TumorObservation    	rdf:type        owl:Class;
						rdfs:label	"p4-lucat:TumorObservation";
						rdfs:subClassOf	 p4-lucat:Observation;
						rdfs:comment "";
						dcterms:modified "2018-11-27"^^xsd:date;
						dcterms:creator <https://www.tib.eu/en/research-development/scientific-data-management/staff/maria-isabel-castellanos/>.

p4-lucat:ToxicityObservation    rdf:type        owl:Class;
						rdfs:label	"p4-lucat:ToxicityObservation";
						rdfs:subClassOf	 p4-lucat:Observation;
						rdfs:comment "";
						dcterms:modified "2019-05-24"^^xsd:date;
						dcterms:creator <https://www.tib.eu/en/research-development/scientific-data-management/staff/maria-isabel-castellanos/>.

p4-lucat:TreatmentLine		rdf:type	owl:Class;
						rdfs:subClassOf p4-lucat:Concept;
						rdfs:label	"TreatmentLine";
						rdfs:comment "Represents any type of treatment line observations.";
						dcterms:modified "2020-12-07"^^xsd:date;
						dcterms:creator <https://www.tib.eu/en/research-development/scientific-data-management/staff/samaneh-jozashoori/>.

p4-lucat:OncologicalTreatmentLine	rdf:type	owl:Class;
							rdfs:subClassOf p4-lucat:TreatmentLine;
							rdfs:label	"OncologicalTreatmentLine";
							rdfs:comment "Represents oncological treatment line observations.";
							dcterms:modified "2020-07-21"^^xsd:date;
							dcterms:creator <https://www.tib.eu/en/research-development/scientific-data-management/staff/samaneh-jozashoori/>.		

p4-lucat:NonOncologicalTreatmentLine	rdf:type	owl:Class;
							rdfs:subClassOf p4-lucat:TreatmentLine;
							rdfs:label	"NonOncologicalTreatmentLine";
							rdfs:comment "Represents non-oncological treatment line observations.";
							dcterms:modified "2020-07-21"^^xsd:date;
							dcterms:creator <https://www.tib.eu/en/research-development/scientific-data-management/staff/samaneh-jozashoori/>.		

p4-lucat:OncologicalSurgery		rdf:type	owl:Class;
							rdfs:subClassOf p4-lucat:Concept;
							rdfs:label	"OncologicalSurgery";
							rdfs:comment "Represents oncological surgery value.";
							dcterms:modified "2020-07-21"^^xsd:date;
							dcterms:creator <https://www.tib.eu/en/research-development/scientific-data-management/staff/samaneh-jozashoori/>.		

p4-lucat:HospitalProcess		rdf:type	owl:Class;
							rdfs:subClassOf p4-lucat:Concept;
							rdfs:label	"HospitalProcess";
							rdfs:comment "Represents the reason of the hospoital service that is provided to the patient. It is identified by the ID of the document from where the service reason is extracted.";
							dcterms:modified "2020-07-21"^^xsd:date;
							dcterms:creator <https://www.tib.eu/en/research-development/scientific-data-management/staff/samaneh-jozashoori/>.	

p4-lucat:HospitalService		rdf:type	owl:Class;
							rdfs:subClassOf p4-lucat:Concept;
							rdfs:label	"HospitalService";
							rdfs:comment "Represents the hospital service that is provided.";
							dcterms:modified "2020-07-21"^^xsd:date;
							dcterms:creator <https://www.tib.eu/en/research-development/scientific-data-management/staff/samaneh-jozashoori/>.																											

p4-lucat:ServiceBeforeDiagnosis		rdf:type	owl:Class;
							rdfs:subClassOf p4-lucat:HospitalService;
							rdfs:label	"ServiceBeforeDiagnosis";
							rdfs:comment "";
							dcterms:modified "2021-02-05"^^xsd:date;
							dcterms:creator <https://www.tib.eu/en/research-development/scientific-data-management/staff/samaneh-jozashoori/>.																											

p4-lucat:ServiceAfterDiagnosis		rdf:type	owl:Class;
							rdfs:subClassOf p4-lucat:HospitalService;
							rdfs:label	"ServiceAfterDiagnosis";
							rdfs:comment "";
							dcterms:modified "2021-02-05"^^xsd:date;
							dcterms:creator <https://www.tib.eu/en/research-development/scientific-data-management/staff/samaneh-jozashoori/>.																											

p4-lucat:ServiceAfterDiagnosisBeforeOncologicalTreatment	rdf:type	owl:Class;
										rdfs:subClassOf p4-lucat:HospitalService;
										rdfs:label	"ServiceAfterDiagnosisBeforeOncologicalTreatment";
										rdfs:comment "";
										dcterms:modified "2021-02-05"^^xsd:date;
										dcterms:creator <https://www.tib.eu/en/research-development/scientific-data-management/staff/samaneh-jozashoori/>.																											

p4-lucat:ServiceDuringOncologicalTreatment	rdf:type	owl:Class;
								rdfs:subClassOf p4-lucat:HospitalService;
								rdfs:label	"ServiceDuringOncologicalTreatment";
								rdfs:comment "";
								dcterms:modified "2021-02-05"^^xsd:date;
								dcterms:creator <https://www.tib.eu/en/research-development/scientific-data-management/staff/samaneh-jozashoori/>.																											

p4-lucat:ServiceAfterOncologicalTreatment	rdf:type	owl:Class;
								rdfs:subClassOf p4-lucat:HospitalService;
								rdfs:label	"ServiceAfterOncologicalTreatment";
								rdfs:comment "";
								dcterms:modified "2021-02-05"^^xsd:date;
								dcterms:creator <https://www.tib.eu/en/research-development/scientific-data-management/staff/samaneh-jozashoori/>.																											

p4-lucat:ScopeOfService		rdf:type	owl:Class;
						rdfs:subClassOf p4-lucat:Concept;
						rdfs:label	"ScopeOfService";
						rdfs:comment "";
						dcterms:modified "2021-02-05"^^xsd:date;
						dcterms:creator <https://www.tib.eu/en/research-development/scientific-data-management/staff/samaneh-jozashoori/>.																											

p4-lucat:TypeOfService		rdf:type	owl:Class;
						rdfs:subClassOf p4-lucat:Concept;
						rdfs:label	"TypeOfService";
						rdfs:comment "";
						dcterms:modified "2021-02-05"^^xsd:date;
						dcterms:creator <https://www.tib.eu/en/research-development/scientific-data-management/staff/samaneh-jozashoori/>.																											

p4-lucat:ServiceDepartment	rdf:type	owl:Class;
						rdfs:subClassOf p4-lucat:Concept;
						rdfs:label	"ServiceDepartment";
						rdfs:comment "";
						dcterms:modified "2021-02-05"^^xsd:date;
						dcterms:creator <https://www.tib.eu/en/research-development/scientific-data-management/staff/samaneh-jozashoori/>.																											

p4-lucat:ProcessComment		rdf:type	owl:Class;
						rdfs:subClassOf p4-lucat:Concept;
						rdfs:label	"ProcessComment";
						rdfs:comment "";
						dcterms:modified "2021-02-05"^^xsd:date;
						dcterms:creator <https://www.tib.eu/en/research-development/scientific-data-management/staff/samaneh-jozashoori/>.																											

p4-lucat:ProcessStatus		rdf:type	owl:Class;
						rdfs:subClassOf p4-lucat:Concept;
						rdfs:label	"ProcessStatus";
						rdfs:comment "";
						dcterms:modified "2021-02-05"^^xsd:date;
						dcterms:creator <https://www.tib.eu/en/research-development/scientific-data-management/staff/samaneh-jozashoori/>.																											

p4-lucat:ClinicalStatus		rdf:type	owl:Class;
						rdfs:subClassOf p4-lucat:Concept;
						rdfs:label	"ClinicalStatus";
						rdfs:comment "";
						dcterms:modified "2021-02-05"^^xsd:date;
						dcterms:creator <https://www.tib.eu/en/research-development/scientific-data-management/staff/samaneh-jozashoori/>.																											

p4-lucat:DiagnosisDescription	rdf:type	owl:Class;
						rdfs:subClassOf p4-lucat:Concept;
						rdfs:label	"DiagnosisDescription";
						rdfs:comment "";
						dcterms:modified "2021-02-05"^^xsd:date;
						dcterms:creator <https://www.tib.eu/en/research-development/scientific-data-management/staff/samaneh-jozashoori/>.																											


#### clinical images:

p4-lucat:Diagnosis  		rdf:type 	owl:Class;
						rdfs:label	"Diagnosis";
						rdfs:subClassOf	p4-lucat:Concept;
						rdfs:comment "The identification of the nature of an illness or other problem by examination of the symptoms.";
						dcterms:modified "2018-11-26"^^xsd:date;
						dcterms:creator <https://www.tib.eu/en/research-development/scientific-data-management/staff/maria-isabel-castellanos/>. 

p4-lucat:LCImage   		rdf:type 	owl:Class;
						rdfs:label	"LCImage";
						rdfs:subClassOf	p4-lucat:Concept;
						rdfs:comment "Image of patient with Lung Cancer";
						dcterms:modified "2018-11-25"^^xsd:date;
						dcterms:creator <https://www.tib.eu/en/research-development/scientific-data-management/staff/maria-isabel-castellanos/>.  

p4-lucat:LungLaterality   	rdf:type 	owl:Class;
						rdfs:label	"LungLaterality";
						rdfs:subClassOf	p4-lucat:Concept;
						rdfs:comment "The laterality of lung to which the image refers.";
						dcterms:modified "2018-11-26"^^xsd:date;
						dcterms:creator <https://www.tib.eu/en/research-development/scientific-data-management/staff/maria-isabel-castellanos/>.

p4-lucat:Modality   		rdf:type 	owl:Class;
						rdfs:label	"Modality";
						rdfs:subClassOf	p4-lucat:Concept;
						rdfs:comment "Modality of image";
						dcterms:modified "2018-11-26"^^xsd:date;
						dcterms:creator <https://www.tib.eu/en/research-development/scientific-data-management/staff/maria-isabel-castellanos/>.

p4-lucat:Organ     		rdf:type 	owl:Class;
						rdfs:label	"Organ";
						rdfs:subClassOf	p4-lucat:Concept;
						rdfs:comment "The organ which the image belong to.";
						dcterms:modified "2018-11-26"^^xsd:date;
						dcterms:creator <https://www.tib.eu/en/research-development/scientific-data-management/staff/maria-isabel-castellanos/>.

p4-lucat:PatientPosition   	rdf:type 	owl:Class;
						rdfs:label	"PatientPosition";
						rdfs:subClassOf	p4-lucat:Concept;
						rdfs:comment "Patient position";
						dcterms:modified "2018-11-26"^^xsd:date;
						dcterms:creator <https://www.tib.eu/en/research-development/scientific-data-management/staff/maria-isabel-castellanos/>.

p4-lucat:BodyPartExamined 	rdf:type        owl:Class;
						rdfs:label	"BodyPartExamined";
						rdfs:subClassOf	p4-lucat:Concept;
						rdfs:comment "";
						dcterms:modified "2018-11-25"^^xsd:date;
						dcterms:creator <https://www.tib.eu/en/research-development/scientific-data-management/staff/maria-isabel-castellanos/>.

####### lc_similarity:

p4-lucat:PatientSimilarity   	rdf:type 	owl:Class;
						rdfs:label	"PatientSimilarity";
						rdfs:subClassOf	p4-lucat:Concept;
						rdfs:comment "";
						dcterms:modified "2018-11-27"^^xsd:date;
						dcterms:creator <https://www.tib.eu/en/research-development/scientific-data-management/staff/maria-isabel-castellanos/>.

##################################################################################################
################################### Properties ###################################################
##################################################################################################


################################### ObjectProperties ###################################################
p4-lucat:CTHasKeyword  		rdf:type 	owl:ObjectProperty;
						rdfs:subPropertyOf owl:topObjectProperty;
						rdfs:domain p4-lucat:ClinicalTrial;
						rdfs:range p4-lucat:Keyword;
						rdfs:comment "This property shows association of clinical trials to medical keywords."@en;
						rdfs:isDefinedBy "emetis_niazmand"@en;
						rdfs:label "CTHasKeyword"@en;
						owl:versionInfo "v1.0"@en.



p4-lucat:CTInPublication  	rdf:type 	owl:ObjectProperty;
                                           	rdfs:subPropertyOf owl:topObjectProperty;
                                           	rdfs:domain p4-lucat:ClinicalTrial;
                                           	rdfs:range p4-lucat:Publication;
                                           	rdfs:comment "This property shows association of clinical trials to scientific publication."@en;
                                           	rdfs:isDefinedBy "emetis_niazmand"@en;
                                           	rdfs:label "CTInPublication"@en;
                                           	owl:versionInfo "v1.0"@en.



p4-lucat:CTOnCondition  	rdf:type 	owl:ObjectProperty;
                                         	rdfs:subPropertyOf owl:topObjectProperty;
                                         	rdfs:domain p4-lucat:ClinicalTrial;
						rdfs:range p4-lucat:Condition;
						rdfs:comment "This property shows association of clinical trials to condition."@en;
						rdfs:isDefinedBy "emetis_niazmand"@en;
						rdfs:label "CTOnCondition"@en;
						owl:versionInfo "v1.0"@en.



p4-lucat:CTOnIntervention  	rdf:type 	owl:ObjectProperty;
                                            	rdfs:subPropertyOf owl:topObjectProperty;
                                            	rdfs:domain p4-lucat:ClinicalTrial;
                                            	rdfs:range p4-lucat:Intervention;
                                            	rdfs:comment "This property shows association of clinical trials to intervention."@en;
                                            	rdfs:isDefinedBy "emetis_niazmand"@en;
                                            	rdfs:label "CTOnIntervention"@en;
                                            	owl:versionInfo "v1.0"@en.


p4-lucat:ConditionInCT  	rdf:type 	owl:ObjectProperty;
                                         	rdfs:subPropertyOf owl:topObjectProperty;
                                         	rdfs:domain p4-lucat:Condition;
                                         	rdfs:range p4-lucat:ClinicalTrial;
                                         	rdfs:comment "This property shows association of condition to clinical trials."@en;
                                         	rdfs:isDefinedBy "emetis_niazmand"@en;
                                         	rdfs:label "ConditionInCT"@en;
                                         	owl:versionInfo "v1.0"@en.



p4-lucat:DesignInterventionModel  rdf:type 	owl:ObjectProperty;
                                                rdfs:subPropertyOf owl:topObjectProperty;
                                                rdfs:domain p4-lucat:ClinicalTrial;
                                                rdfs:range p4-lucat:Assignment;
                                                rdfs:comment "This property shows association of clinical trials to assignment (e.g., Single or Parallel Assignment)."@en;
                                                rdfs:isDefinedBy "emetis_niazmand"@en;
                                                rdfs:label "DesignInterventionModel"@en;
                                                owl:versionInfo "v1.0"@en.


p4-lucat:GenderInCT  		rdf:type 	owl:ObjectProperty;
					      	rdfs:subPropertyOf owl:topObjectProperty;
					      	rdfs:domain p4-lucat:ClinicalTrial;
					      	rdfs:range p4-lucat:Gender;
					      	rdfs:comment "This property shows association of clinical trials to gender."@en;
					      	rdfs:isDefinedBy "emetis_niazmand"@en;
					      	rdfs:label "GenderInCT"@en;
					      	owl:versionInfo "v1.0"@en.


p4-lucat:InterventionInCT  	rdf:type 	owl:ObjectProperty;
                                            	rdfs:subPropertyOf owl:topObjectProperty;
                                            	rdfs:domain p4-lucat:Intervention;
                                            	rdfs:range p4-lucat:ClinicalTrial;
                                            	rdfs:comment "This property shows association of intervention to clinical trials."@en;
                                            	rdfs:isDefinedBy "emetis_niazmand"@en;
                                            	rdfs:label "InterventionInCT"@en;
                                            	owl:versionInfo "v1.0"@en.


p4-lucat:KeywordMentionedInCT  rdf:type 	owl:ObjectProperty;
                                                rdfs:subPropertyOf owl:topObjectProperty;
                                                rdfs:domain p4-lucat:Keyword;
                                                rdfs:range p4-lucat:ClinicalTrial;
                                                rdfs:comment "This property shows association of medical keywords to clinical trials."@en;
                                                rdfs:isDefinedBy "emetis_niazmand"@en;
                                                rdfs:label "KeywordMentionedInCT"@en;
                                                owl:versionInfo "v1.0"@en.


p4-lucat:PubOfCT  		rdf:type 	owl:ObjectProperty;
					   	rdfs:subPropertyOf owl:topObjectProperty;
					   	rdfs:domain p4-lucat:Publication;
					   	rdfs:range p4-lucat:ClinicalTrial;
					   	rdfs:comment "This property shows association of scientific publication to clinical trials."@en;
					   	rdfs:isDefinedBy "emetis_niazmand"@en;
					   	rdfs:label "PubOfCT"@en;
					   	owl:versionInfo "v1.0"@en.

p4-lucat:Egfr  			rdf:type 	owl:ObjectProperty;
					   	rdfs:domain p4-lucat:ClinicalTrial;
					   	rdfs:range p4-lucat:EGFR;
					   	rdfs:comment "This property shows association of biomarker egfr to clinical trials."@en;
					   	rdfs:isDefinedBy "emetis_niazmand"@en;
					   	rdfs:label "Egfr"@en;
					   	owl:versionInfo "v1.0"@en.

p4-lucat:Alk  			rdf:type 	owl:ObjectProperty;
					   	rdfs:domain p4-lucat:ClinicalTrial;
					   	rdfs:range p4-lucat:ALK;
					   	rdfs:comment "This property shows association of biomarker alk to clinical trials."@en;
					   	rdfs:isDefinedBy "emetis_niazmand"@en;
					   	rdfs:label "alk"@en;
					   	owl:versionInfo "v1.0"@en.

p4-lucat:Ros1  			rdf:type 	owl:ObjectProperty;
					   	rdfs:domain p4-lucat:ClinicalTrial;
					   	rdfs:range p4-lucat:ROS;
					   	rdfs:comment "This property shows association of biomarker ros1 to clinical trials."@en;
					   	rdfs:isDefinedBy "emetis_niazmand"@en;
					   	rdfs:label "ros1"@en;
					   	owl:versionInfo "v1.0"@en.

p4-lucat:Radiotherapy  		rdf:type 	owl:ObjectProperty;
					   	rdfs:domain p4-lucat:ClinicalTrial;
					   	rdfs:range p4-lucat:Radiotherapy;
					   	rdfs:comment "This property shows association of Radiotherapy to clinical trials."@en;
					   	rdfs:isDefinedBy "emetis_niazmand"@en;
					   	rdfs:label "Radiotherapy"@en;
					   	owl:versionInfo "v1.0"@en.

p4-lucat:Tki  			rdf:type 	owl:ObjectProperty;
					   	rdfs:domain p4-lucat:ClinicalTrial;
					   	rdfs:range p4-lucat:TKI;
					   	rdfs:comment "This property shows association of tki to clinical trials."@en;
					   	rdfs:isDefinedBy "emetis_niazmand"@en;
					   	rdfs:label "tki"@en;
					   	owl:versionInfo "v1.0"@en.

p4-lucat:Chemotherapy  		rdf:type 	owl:ObjectProperty;
					   	rdfs:domain p4-lucat:ClinicalTrial;
					   	rdfs:range p4-lucat:Chemotherapy;
					   	rdfs:comment "This property shows association of Chemotherapy to clinical trials."@en;
					   	rdfs:isDefinedBy "emetis_niazmand"@en;
					   	rdfs:label "Chemotherapy"@en;
					   	owl:versionInfo "v1.0"@en.

p4-lucat:Immunotherapy  	rdf:type 	owl:ObjectProperty;
					   	rdfs:domain p4-lucat:ClinicalTrial;
					   	rdfs:range p4-lucat:Immunotherapy;
					   	rdfs:comment "This property shows association of Immunotherapy to clinical trials."@en;
					   	rdfs:isDefinedBy "emetis_niazmand"@en;
					   	rdfs:label "Immunotherapy"@en;
					   	owl:versionInfo "v1.0"@en.

p4-lucat:Surgery  		rdf:type 	owl:ObjectProperty;
					   	rdfs:domain p4-lucat:ClinicalTrial;
					   	rdfs:range p4-lucat:Surgery;
					   	rdfs:comment "This property shows association of Surgery to clinical trials."@en;
					   	rdfs:isDefinedBy "emetis_niazmand"@en;
					   	rdfs:label "Surgery"@en;
					   	owl:versionInfo "v1.0"@en.

p4-lucat:Antiangiogenic  	rdf:type 	owl:ObjectProperty;
					   	rdfs:domain p4-lucat:ClinicalTrial;
					   	rdfs:range p4-lucat:Antiangiogenic;
					   	rdfs:comment "This property shows association of Antiangiogenic to clinical trials."@en;
					   	rdfs:isDefinedBy "emetis_niazmand"@en;
					   	rdfs:label "Antiangiogenic"@en;
					   	owl:versionInfo "v1.0"@en.

p4-lucat:Stages  		rdf:type 	owl:ObjectProperty;
					   	rdfs:domain p4-lucat:ClinicalTrial;
					   	rdfs:range p4-lucat:Stages;
					   	rdfs:comment "This property shows association of Stages to clinical trials."@en;
					   	rdfs:isDefinedBy "emetis_niazmand"@en;
					   	rdfs:label "Stages"@en;
					   	owl:versionInfo "v1.0"@en.

p4-lucat:PerformanceObservation  	rdf:type 	owl:ObjectProperty;
					   	rdfs:domain p4-lucat:ClinicalTrial;
					   	rdfs:range p4-lucat:PerformanceObservation;
					   	rdfs:comment "This property shows association of PerformanceObservation to clinical trials."@en;
					   	rdfs:isDefinedBy "emetis_niazmand"@en;
					   	rdfs:label "PerformanceObservation"@en;
					   	owl:versionInfo "v1.0"@en.
#### WP4 requirements:

p4-lucat:provenance		rdf:type	owl:ObjectProperty;
						rdfs:label	"provenance";
						rdfs:domain p4-lucat:Concept;
						rdfs:range	p4-lucat:SourceName;
						rdfs:comment	"The name of the source from which the concept is extracted or derived";
						dcterms:modified "2017-11-23"^^xsd:date;
						dcterms:creator <https://www.tib.eu/en/research-development/scientific-data-management/staff/>.

p4-lucat:hasAnnotation		rdf:type 	owl:ObjectProperty;
						rdfs:label	"hasAnnotation";
						rdfs:domain p4-lucat:Relation;
				  		rdfs:range p4-lucat:Annotation;
						rdfs:comment	"Connection between the annotation and the relation between annotation and publication";
						dcterms:modified "2019-01-30"^^xsd:date;
						dcterms:creator <https://www.tib.eu/en/research-development/scientific-data-management/staff/samaneh-jozashoori/>.

p4-lucat:hasCUIAnnotation	rdf:type 	owl:ObjectProperty;
						rdfs:label	"hasCUIAnnotation";
						rdfs:domain p4-lucat:Concept;
				  		rdfs:range p4-lucat:Annotation;
						rdfs:comment	"CUI annotation of the concept.";
						dcterms:modified "2019-01-29"^^xsd:date;
						dcterms:creator <https://www.tib.eu/en/research-development/scientific-data-management/staff/samaneh-jozashoori/>.


p4-lucat:hasHPOAnnotation	rdf:type 	owl:ObjectProperty;
						rdfs:label	"hasHPOAnnotation";
						rdfs:domain p4-lucat:Phenotype;
				  		rdfs:range p4-lucat:Annotation;
						rdfs:comment	"HPO annotation of the phenotype.";
						dcterms:modified "2019-01-30"^^xsd:date;
						dcterms:creator <https://www.tib.eu/en/research-development/scientific-data-management/staff/samaneh-jozashoori/>.

p4-lucat:author			rdf:type	owl:ObjectProperty;
						rdfs:label	"authors";
						rdfs:domain	p4-lucat:Publication;
						rdfs:range	p4-lucat:Author;
						rdfs:comment	"Authors of publication";
						dcterms:modified "2019-05-24"^^xsd:date;
						dcterms:creator <https://www.tib.eu/en/research-development/scientific-data-management/staff/samaneh-jozashoori/>.

p4-lucat:annotates		rdf:type	owl:ObjectProperty;
						rdfs:label	"annotates";
						rdfs:domain	p4-lucat:Relation;
						rdfs:range	p4-lucat:Publication;
						rdfs:comment	"Connection between mentionedIn or HasTopic relation with CUI.";
						dcterms:modified "2019-05-24"^^xsd:date;
						dcterms:creator <https://www.tib.eu/en/research-development/scientific-data-management/staff/samaneh-jozashoori/>.

p4-lucat:publication_isRelatedTo_Disease	rdf:type	owl:ObjectProperty;
								rdfs:label	"publication_isRelatedTo_Disease";
								rdfs:domain	p4-lucat:Publication;
								rdfs:range	p4-lucat:Disorder;
								rdfs:comment	"";
								dcterms:modified "2019-05-24"^^xsd:date;
								dcterms:creator <https://www.tib.eu/en/research-development/scientific-data-management/staff/samaneh-jozashoori/>.

p4-lucat:relation_isRelatedTo_annotation	rdf:type        owl:ObjectProperty;	
				                		rdfs:label	"relation_isRelatedTo_annotation";
								rdfs:domain	p4-lucat:Relation;
								rdfs:range	p4-lucat:Annotation;
								rdfs:comment	".";
								dcterms:modified "2018-11-27"^^xsd:date;
								dcterms:creator <https://www.tib.eu/en/research-development/scientific-data-management/staff/maria-isabel-castellanos/>.


p4-lucat:relation_isRelatedTo_publication	rdf:type        owl:ObjectProperty;	
				                		rdfs:label	"relation_isRelatedTo_publication";
								rdfs:domain	p4-lucat:Relation;
								rdfs:range	p4-lucat:Publication;
								rdfs:comment	".";
								dcterms:modified "2019-05-24"^^xsd:date;
								dcterms:creator <https://www.tib.eu/en/research-development/scientific-data-management/staff/maria-isabel-castellanos/>.

p4-lucat:annotation_isRelatedTo_Disease		rdf:type        owl:ObjectProperty;	
					                	rdfs:label	"annotation_isRelatedTo_Disease";
								rdfs:domain	p4-lucat:Annotation;
								rdfs:range	p4-lucat:Disorder;
								rdfs:comment ".";
								dcterms:modified "2020-10-29"^^xsd:date;
								dcterms:creator <https://www.tib.eu/en/research-development/scientific-data-management/staff/samaneh-jozashoori/>.

p4-lucat:relation_isRelatedTo_Disease		rdf:type 	owl:ObjectProperty;	
					                	rdfs:label	"relation_isRelatedTo_Disease";
								rdfs:domain	p4-lucat:Relation;
								rdfs:range	p4-lucat:Disorder;
								rdfs:comment ".";
								dcterms:modified "2020-10-29"^^xsd:date;
								dcterms:creator <https://www.tib.eu/en/research-development/scientific-data-management/staff/samaneh-jozashoori/>.

p4-lucat:hasTopicRelation_isRelatedTo_Disease	rdf:type 	owl:ObjectProperty;	
							        rdfs:label	"hasTopicRelation_isRelatedTo_Disease";
								rdfs:domain	p4-lucat:HAS_TOPIC;
								rdfs:range	p4-lucat:Disorder;
								rdfs:comment ".";
								dcterms:modified "2020-10-29"^^xsd:date;
								dcterms:creator <https://www.tib.eu/en/research-development/scientific-data-management/staff/samaneh-jozashoori/>.									

p4-lucat:mentionedInRelation_isRelatedTo_Disease	rdf:type 	owl:ObjectProperty;	
								        rdfs:label	"mentionedInRelation_isRelatedTo_Disease";
									rdfs:domain	p4-lucat:MENTIONED_IN;
									rdfs:range	p4-lucat:Disorder;
									rdfs:comment ".";
									dcterms:modified "2020-10-29"^^xsd:date;
									dcterms:creator <https://www.tib.eu/en/research-development/scientific-data-management/staff/samaneh-jozashoori/>.

p4-lucat:hasAuthor		rdf:type 	owl:ObjectProperty;	
               	 				rdfs:label	"hasAuthor";
						rdfs:domain	p4-lucat:Publication;
						rdfs:range	p4-lucat:Author;
						rdfs:comment ".";
						dcterms:modified "2020-10-29"^^xsd:date;
						dcterms:creator <https://www.tib.eu/en/research-development/scientific-data-management/staff/samaneh-jozashoori/>.

p4-lucat:hasPublicationType	rdf:type owl:ObjectProperty;	
		                rdfs:label	"hasPublicationType";
						rdfs:domain	p4-lucat:Publication;
						rdfs:range	p4-lucat:PublicationType;
						rdfs:comment ".";
						dcterms:modified "2020-10-29"^^xsd:date;
						dcterms:creator <https://www.tib.eu/en/research-development/scientific-data-management/staff/samaneh-jozashoori/>.

#### Drug requirements:

p4-lucat:drugDrugInteraction	rdf:type	owl:ObjectProperty;
								rdfs:label	"drug_interactsWith_drug";
								rdfs:domain	p4-lucat:Drug;
								rdfs:range	p4-lucat:Drug;
								rdfs:comment	"Represents drug-drug interactions.";
								dcterms:modified "2018-07-24"^^xsd:date;
								dcterms:creator <https://www.tib.eu/en/research-development/scientific-data-management/staff/samaneh-jozashoori/>.									

p4-lucat:drug_isRelatedTo_dse	rdf:type	owl:ObjectProperty;
							rdfs:label	"drug_isRelatedTo_dse";
							rdfs:domain	p4-lucat:Drug;
							rdfs:range	p4-lucat:DrugSideEffect;
							rdfs:comment	"Connection between drug and drug-sideEffect relation.";
							dcterms:modified "2018-07-24"^^xsd:date;
							dcterms:creator <https://www.tib.eu/en/research-development/scientific-data-management/staff/samaneh-jozashoori/>.

p4-lucat:sideEffect_isRelatedTo_dse	rdf:type	owl:ObjectProperty;
									rdfs:label	"sideEffect_isRelatedTo_dse";
									rdfs:domain	p4-lucat:Phenotype;
									rdfs:range	p4-lucat:DrugSideEffect;
									rdfs:comment	"Connection between sideEffect and drug-sideEffect relation.";
									dcterms:modified "2018-07-24"^^xsd:date;
									dcterms:creator <https://www.tib.eu/en/research-development/scientific-data-management/staff/samaneh-jozashoori/>.

p4-lucat:affects	rdf:type	owl:ObjectProperty;
								rdfs:label	"affects";
								rdfs:domain	p4-lucat:EffectInteraction;
								rdfs:range	p4-lucat:Drug;
								rdfs:comment	"The conncetion between drug that affects by the other one through their interaction and the interaction node.";
								dcterms:modified "2018-11-27"^^xsd:date;
								dcterms:creator <https://www.tib.eu/en/research-development/scientific-data-management/staff/samaneh-jozashoori/>.

p4-lucat:isAffected	rdf:type	owl:ObjectProperty;
								rdfs:label	"isAffected";
								rdfs:domain	p4-lucat:EffectInteraction;
								rdfs:range	p4-lucat:Drug;
								rdfs:comment	"The conncetion between drug that is affected by the other one through their interaction and the interaction node.";
								dcterms:modified "2018-11-27"^^xsd:date;
								dcterms:creator <https://www.tib.eu/en/research-development/scientific-data-management/staff/samaneh-jozashoori/>.

p4-lucat:enzyme_isRelatedTo_gene	rdf:type	owl:ObjectProperty;
									rdfs:label	"enzyme_isRelatedTo_gene";
									rdfs:domain	p4-lucat:Enzyme;
									rdfs:range	p4-lucat:Gene;
									rdfs:comment	"The connection between the enzyme and the gene from which it is produced.";
									dcterms:modified "2018-10-30"^^xsd:date;
									dcterms:creator <https://www.tib.eu/en/research-development/scientific-data-management/staff/samaneh-jozashoori/>.

p4-lucat:target_isRelatedTo_gene	rdf:type	owl:ObjectProperty;
									rdfs:label	"target_isRelatedTo_gene";
									rdfs:domain	p4-lucat:Target;
									rdfs:range	p4-lucat:Gene;
									rdfs:comment	"The connection between the target and the gene from which it is produced.";
									dcterms:modified "2018-10-30"^^xsd:date;
									dcterms:creator <https://www.tib.eu/en/research-development/scientific-data-management/staff/samaneh-jozashoori/>.

p4-lucat:biomarker_has_indication	rdf:type	owl:ObjectProperty;
								rdfs:label	"biomarker_has_indication";
								rdfs:domain	p4-lucat:Biomarker;
								rdfs:range	p4-lucat:Drug;
								rdfs:comment	"";
								dcterms:modified "2019-01-07"^^xsd:date;
								dcterms:creator <https://www.tib.eu/en/research-development/scientific-data-management/staff/samaneh-jozashoori/>.

p4-lucat:tumorStage_has_indication	rdf:type	owl:ObjectProperty;
								rdfs:label	"tumorStage_has_indication";
								rdfs:domain	p4-lucat:TumorStage;
								rdfs:range	p4-lucat:Drug;
								rdfs:comment	"";
								dcterms:modified "2019-01-07"^^xsd:date;
								dcterms:creator <https://www.tib.eu/en/research-development/scientific-data-management/staff/samaneh-jozashoori/>.

p4-lucat:object_drug	rdf:type	owl:ObjectProperty;
							rdfs:label	"object_drug";
							rdfs:domain	p4-lucat:DrugDrugInteraction;
							rdfs:range	p4-lucat:Drug;
							rdfs:comment	"Relation which connects the drug drug interacion to the object drug.";
							dcterms:modified "2020-07-24"^^xsd:date;
							dcterms:creator <https://www.tib.eu/en/research-development/scientific-data-management/staff/samaneh-jozashoori/>.	

p4-lucat:effect	rdf:type	owl:ObjectProperty;
							rdfs:label	"effect";
							rdfs:domain	p4-lucat:DrugDrugInteraction;
							rdfs:range	p4-lucat:AdverseEvent;
							rdfs:comment	"The relationship between the drug drug interaction and corresponding adverse event.";
							dcterms:modified "2020-09-14"^^xsd:date;
							dcterms:creator <https://www.tib.eu/en/research-development/scientific-data-management/staff/samaneh-jozashoori/>.								

p4-lucat:precipitant_drug	rdf:type	owl:ObjectProperty;
							rdfs:label	"precipitant_drug";
							rdfs:domain	p4-lucat:DrugDrugInteraction;
							rdfs:range	p4-lucat:Drug;
							rdfs:comment	"Relation which connects the drug drug interacion to the precipitant drug.";
							dcterms:modified "2020-07-24"^^xsd:date;
							dcterms:creator <https://www.tib.eu/en/research-development/scientific-data-management/staff/samaneh-jozashoori/>.										

p4-lucat:interactor1	rdf:type	owl:ObjectProperty;
							rdfs:label	"interactor1";
							rdfs:domain	p4-lucat:Interaction;
							rdfs:range	p4-lucat:Drug;
							rdfs:comment	"Relation which connects an interaction to the involved drug.";
							dcterms:modified "2020-07-24"^^xsd:date;
							dcterms:creator <https://www.tib.eu/en/research-development/scientific-data-management/staff/samaneh-jozashoori/>.

p4-lucat:interactor2	rdf:type	owl:ObjectProperty;
							rdfs:label	"interactor2";
							rdfs:domain	p4-lucat:Interaction;
							rdfs:range	p4-lucat:Concept;
							rdfs:comment	"Relation which connects an interacion to the second involved concept (e.g. disorder, enzyme,...).";
							dcterms:modified "2020-07-24"^^xsd:date;
							dcterms:creator <https://www.tib.eu/en/research-development/scientific-data-management/staff/samaneh-jozashoori/>.							

p4-lucat:interaction_isRelatedTo_Disease	rdf:type	owl:ObjectProperty;
										rdfs:label	"interaction_isRelatedTo_Disease";
										rdfs:domain	p4-lucat:Interaction;
										rdfs:range	p4-lucat:Disorder;
										rdfs:comment	"Connection between the interaction and disease.";
										dcterms:modified "2020-10-29"^^xsd:date;
										dcterms:creator <https://www.tib.eu/en/research-development/scientific-data-management/staff/samaneh-jozashoori/>.	

#### WP2 requirements:
##### lc_notes:
p4-lucat:hasPerformanceStatus	rdf:type        owl:ObjectProperty;	
						rdfs:label	"hasPerformanceStatus";
						rdfs:domain	p4-lucat:PerformanceObservation;
						rdfs:range	p4-lucat:PerformanceStatus;
						rdfs:comment	"Connection between patient with lung cancer and performance status observations.";
						dcterms:modified "2018-11-27"^^xsd:date;
						dcterms:creator <https://www.tib.eu/en/research-development/scientific-data-management/staff/samaneh-jozashoori/>.

p4-lucat:hasTki	rdf:type        owl:ObjectProperty;	
				rdfs:label	"hasTki";
						rdfs:domain	p4-lucat:LCPatient;
						rdfs:range	p4-lucat:Drug;
						rdfs:comment	"Connection between patient with lung cancer and the tki drugs that has been prescribed.";
						dcterms:modified "2018-11-27"^^xsd:date;
						dcterms:creator <https://www.tib.eu/en/research-development/scientific-data-management/staff/samaneh-jozashoori/>.

p4-lucat:hasImmunotherapy	rdf:type        owl:ObjectProperty;	
				rdfs:label	"hasImmunotherapy";
						rdfs:domain	p4-lucat:LCPatient;
						rdfs:range	p4-lucat:Drug;
						rdfs:comment	"Connection between patient with lung cancer and the immunotherapy drugs that has been prescribed.";
						dcterms:modified "2018-11-27"^^xsd:date;
						dcterms:creator <https://www.tib.eu/en/research-development/scientific-data-management/staff/samaneh-jozashoori/>.

p4-lucat:hasFamiliarAntecedent	rdf:type        owl:ObjectProperty;	
				rdfs:label	"hasFamiliarAntecedent";
						rdfs:domain	p4-lucat:LCPatient;
						rdfs:range	p4-lucat:FamiliarAntecedent;
						rdfs:comment	"Connection between patient with lung cancer and her/his familiar antecedents.";
						dcterms:modified "2018-11-27"^^xsd:date;
						dcterms:creator <https://www.tib.eu/en/research-development/scientific-data-management/staff/samaneh-jozashoori/>.

p4-lucat:hasDrugGroup	rdf:type        owl:ObjectProperty;	
				rdfs:label	"hasDrug";
						rdfs:domain	p4-lucat:LCPatient;
						rdfs:range	p4-lucat:DrugGroup;
						rdfs:comment	"Connection between patient with lung cancer and the types of drugs that has been prescribed.";
						dcterms:modified "2017-10-04"^^xsd:date;
						dcterms:creator <https://www.tib.eu/en/research-development/scientific-data-management/staff/samaneh-jozashoori/>.


p4-lucat:hasComorbidity	rdf:type        owl:ObjectProperty;	
				rdfs:label	"hasComorbidity";
						rdfs:domain	p4-lucat:LCPatient;
						rdfs:range	p4-lucat:Disorder;
						rdfs:comment	"Connection between patient with lung cancer and her/his Comorbidities.";
						dcterms:modified "2018-11-27"^^xsd:date;
						dcterms:creator <https://www.tib.eu/en/research-development/scientific-data-management/staff/samaneh-jozashoori/>.

p4-lucat:hasChemotherapy	rdf:type        owl:ObjectProperty;	
				rdfs:label	"hasChemotherapy";
						rdfs:domain	p4-lucat:LCPatient;
						rdfs:range	p4-lucat:Drug;
						rdfs:comment	"Connection between patient with lung cancer and the Chemotherapy drugs that has been prescribed.";
						dcterms:modified "2018-11-27"^^xsd:date;
						dcterms:creator <https://www.tib.eu/en/research-development/scientific-data-management/staff/samaneh-jozashoori/>.

p4-lucat:hasLiquidBiopsy	rdf:type        owl:ObjectProperty;	
				rdfs:label	"hasLiquidBiopsy";
						rdfs:domain	p4-lucat:LCPatient;
						rdfs:range	p4-lucat:LiquidBiopsy;
						rdfs:comment	"Connection between patient with lung cancer and the liquid biopsy tests that has been run.";
						dcterms:modified "2017-10-04"^^xsd:date;
						dcterms:creator <https://www.tib.eu/en/research-development/scientific-data-management/staff/samaneh-jozashoori/>.

p4-lucat:hasMutation	rdf:type        owl:ObjectProperty;	
				rdfs:label	"hasMutation";
						rdfs:domain	p4-lucat:LiquidBiopsy;
						rdfs:range	p4-lucat:Mutation;
						rdfs:comment	"Connection between liquid biopsy test and the mutation that has been observed.";
						dcterms:modified "2017-10-04"^^xsd:date;
						dcterms:creator <https://www.tib.eu/en/research-development/scientific-data-management/staff/samaneh-jozashoori/>.

p4-lucat:hasPerformanceObservation	rdf:type        owl:ObjectProperty;	
				rdfs:label	"hasPerformanceObservation";
						rdfs:domain	p4-lucat:LCPatient;
						rdfs:range	p4-lucat:PerformanceObservation;
						rdfs:comment	"";
						dcterms:modified "2019-01-30"^^xsd:date;
						dcterms:creator <https://www.tib.eu/en/research-development/scientific-data-management/staff/samaneh-jozashoori/>.

p4-lucat:gender	rdf:type	owl:ObjectProperty;
				rdfs:label	"gender";
				rdfs:domain	p4-lucat:LCPatient;
				rdfs:range	p4-lucat:Gender;
				rdfs:comment	"Gender value of the patient.";
				dcterms:modified "2018-01-14"^^xsd:date;
				dcterms:creator <https://www.tib.eu/en/research-development/scientific-data-management/staff/samaneh-jozashoori/>.

p4-lucat:tumorType	rdf:type	owl:ObjectProperty;
				rdfs:label	"tumorType";
				rdfs:domain	p4-lucat:LCPatient;
				rdfs:range	p4-lucat:TumorType;
				rdfs:comment	"tumorType";
				dcterms:modified "2019-01-30"^^xsd:date;
				dcterms:creator <https://www.tib.eu/en/research-development/scientific-data-management/staff/samaneh-jozashoori/>.

p4-lucat:hasTumorStage	rdf:type        owl:ObjectProperty;	
				rdfs:label	"hasTumorStage";
						rdfs:domain	p4-lucat:TumorObservation;
						rdfs:range	p4-lucat:TumorStage;
						rdfs:comment	".";
						dcterms:modified "2018-11-27"^^xsd:date;
						dcterms:creator <https://www.tib.eu/en/research-development/scientific-data-management/staff/maria-isabel-castellanos/>.

p4-lucat:hasTumorObservation	rdf:type        owl:ObjectProperty;	
				rdfs:label	"hasTumorObservation";
						rdfs:domain	p4-lucat:LCPatient;
						rdfs:range	p4-lucat:TumorObservation;
						rdfs:comment	".";
						dcterms:modified "2019-01-30"^^xsd:date;
						dcterms:creator <https://www.tib.eu/en/research-development/scientific-data-management/staff/samaneh-jozashoori/>.

p4-lucat:hasToxicityObservation	rdf:type        owl:ObjectProperty;	
				rdfs:label	"hasToxicityObservation";
						rdfs:domain	p4-lucat:LCPatient;
						rdfs:range	p4-lucat:ToxicityObservation;
						rdfs:comment ".";
						dcterms:modified "2019-05-24"^^xsd:date;
						dcterms:creator  <https://www.tib.eu/en/research-development/scientific-data-management/staff/maria-isabel-castellanos/>.

p4-lucat:hasToxicity	rdf:type        owl:ObjectProperty;	
				rdfs:label	"hasToxicity";
						rdfs:domain	p4-lucat:ToxicityObservation;
						rdfs:range	p4-lucat:Phenotype;
						rdfs:comment	".";
						dcterms:modified "2019-05-24"^^xsd:date;
						dcterms:creator  <https://www.tib.eu/en/research-development/scientific-data-management/staff/maria-isabel-castellanos/>.

p4-lucat:hasNonOncologicalDrug	rdf:type        owl:ObjectProperty;	
				        rdfs:label	"hasNonOncologicalDrug";
						rdfs:domain	p4-lucat:LCPatient;
						rdfs:range	p4-lucat:Drug;
						rdfs:comment "Relation between the patient and the non-oncological line of treamtment.";
						dcterms:modified "2020-07-21"^^xsd:date;
						dcterms:creator <https://www.tib.eu/en/research-development/scientific-data-management/staff/samaneh-jozashoori/>.	

p4-lucat:hasNonOncologicalDrugInFirstTreatmentLine	rdf:type        owl:ObjectProperty;	
										        rdfs:label	"hasNonOncologicalDrugInFirstTreatmentLine";
										        rdfs:subPropertyOf p4-lucat:hasNonOncologicalDrug;
												rdfs:domain	p4-lucat:LCPatient;
												rdfs:range	p4-lucat:Drug;
												rdfs:comment "Relation between the patient and the non-oncological drug which is prescibed before/during the first oncological line of treamtment.";
												dcterms:modified "2020-11-13"^^xsd:date;
												dcterms:creator <https://www.tib.eu/en/research-development/scientific-data-management/staff/samaneh-jozashoori/>.	

p4-lucat:hasOncologicalTreatmentLine	rdf:type        owl:ObjectProperty;	
				        rdfs:label	"hasOncologicalTreatmentLine";
						rdfs:domain	p4-lucat:LCPatient;
						rdfs:range	p4-lucat:OncologicalTreatmentLine;
						rdfs:comment "Relation between the patient and the oncological line of treamtment.";
						dcterms:modified "2020-07-21"^^xsd:date;
						dcterms:creator <https://www.tib.eu/en/research-development/scientific-data-management/staff/samaneh-jozashoori/>.	

p4-lucat:treatment_has_oncologicalDrug	rdf:type        owl:ObjectProperty;	
				        rdfs:label	"treatment_has_oncologicalDrug";
						rdfs:domain	p4-lucat:OncologicalTreatmentLine;
						rdfs:range	p4-lucat:Drug;
						rdfs:comment "Relation between the treatment line and the oncological drugs.";
						dcterms:modified "2020-07-22"^^xsd:date;
						dcterms:creator <https://www.tib.eu/en/research-development/scientific-data-management/staff/samaneh-jozashoori/>.		

p4-lucat:treatment_has_nonOncologicalDrug	rdf:type        owl:ObjectProperty;	
				        rdfs:label	"treatmentInitDate";
						rdfs:domain	p4-lucat:NonOncologicalTreatmentLine;
						rdfs:range	p4-lucat:Drug;
						rdfs:comment "Relation between the treatment line and the non-oncological drugs.";
						dcterms:modified "2020-07-21"^^xsd:date;
						dcterms:creator <https://www.tib.eu/en/research-development/scientific-data-management/staff/samaneh-jozashoori/>.																																																								

p4-lucat:hasOncologicalSurgery	rdf:type        owl:ObjectProperty;	
				        rdfs:label	"hasOncologicalSurgery";
						rdfs:domain	p4-lucat:LCPatient;
						rdfs:range	p4-lucat:OncologicalSurgery;
						rdfs:comment "Relation between the patient and the surgey that has been performed on.";
						dcterms:modified "2020-07-21"^^xsd:date;
						dcterms:creator <https://www.tib.eu/en/research-development/scientific-data-management/staff/samaneh-jozashoori/>.							

p4-lucat:hasHospitalProcess	rdf:type        owl:ObjectProperty;	
				        rdfs:label	"hasHospitalProcess";
						rdfs:domain	p4-lucat:LCPatient;
						rdfs:range	p4-lucat:HospitalProcess;
						rdfs:comment "Relation between the patient to which the hospital process belongs and the hospital process.";
						dcterms:modified "2020-07-21"^^xsd:date;
						dcterms:creator <https://www.tib.eu/en/research-development/scientific-data-management/staff/samaneh-jozashoori/>.																							

p4-lucat:hasHospitalService	rdf:type        owl:ObjectProperty;	
						        rdfs:label	"hasHospitalService";
								rdfs:domain	p4-lucat:LCPatient;
								rdfs:range	p4-lucat:HospitalService;
								rdfs:comment "";
								dcterms:modified "2020-12-21"^^xsd:date;
								dcterms:creator <https://www.tib.eu/en/research-development/scientific-data-management/staff/samaneh-jozashoori/>.	
##### lc_images:
p4-lucat:hasImage       rdf:type     owl:ObjectProperty;
							rdfs:label	"hasImage";
							rdfs:domain	p4-lucat:LCPatient;
							rdfs:range	p4-lucat:LCImage;
							rdfs:comment ".";
							dcterms:modified "2018-11-27"^^xsd:date;
							dcterms:creator <https://www.tib.eu/en/research-development/scientific-data-management/staff/maria-isabel-castellanos/>.

p4-lucat:imageType      rdf:type     owl:ObjectProperty;
							rdfs:label	"imageType";
							rdfs:domain	p4-lucat:LCImage;
							rdfs:range	rdfs:Literal;
							rdfs:comment ".";
							dcterms:modified "2019-01-30"^^xsd:date;
							dcterms:creator <https://www.tib.eu/en/research-development/scientific-data-management/staff/samaneh-jozashoori/>.

p4-lucat:modality      rdf:type     owl:ObjectProperty;
							rdfs:label	"modality";
							rdfs:domain	p4-lucat:LCImage;
							rdfs:range	p4-lucat:Modality;
							rdfs:comment ".";
							dcterms:modified "2018-11-27"^^xsd:date;
							dcterms:creator <https://www.tib.eu/en/research-development/scientific-data-management/staff/maria-isabel-castellanos/>.

p4-lucat:bodyPartExamined      rdf:type     owl:ObjectProperty;
							rdfs:label	"bodyPartExamined";
							rdfs:domain	p4-lucat:LCImage;
							rdfs:range	p4-lucat:BodyPartExamined;
							rdfs:comment ".";
							dcterms:modified "2018-11-25"^^xsd:date;
							dcterms:creator <https://www.tib.eu/en/research-development/scientific-data-management/staff/maria-isabel-castellanos/>.

p4-lucat:patientPosition      rdf:type     owl:ObjectProperty;
							rdfs:label	"patientPosition";
							rdfs:domain	p4-lucat:LCImage;
							rdfs:range	p4-lucat:PatientPosition;
							rdfs:comment ".";
							dcterms:modified "2018-11-27"^^xsd:date;
							dcterms:creator <https://www.tib.eu/en/research-development/scientific-data-management/staff/maria-isabel-castellanos/>.

p4-lucat:lungLaterality      rdf:type     owl:ObjectProperty;
							rdfs:label	"lungLaterality";
							rdfs:domain	p4-lucat:Organ;
							rdfs:range	p4-lucat:LungLaterality;
							rdfs:comment ".";
							dcterms:modified "2018-11-27"^^xsd:date;
							dcterms:creator <https://www.tib.eu/en/research-development/scientific-data-management/staff/maria-isabel-castellanos/>.

p4-lucat:hasOrgans     rdf:type     owl:ObjectProperty;
							rdfs:label	"hasOrgans";
							rdfs:domain	p4-lucat:LCImage;
							rdfs:range	p4-lucat:Organ;
							rdfs:comment ".";
							dcterms:modified "2018-11-27"^^xsd:date;
							dcterms:creator <https://www.tib.eu/en/research-development/scientific-data-management/staff/maria-isabel-castellanos/>.

p4-lucat:hasDiagnosis     rdf:type     owl:ObjectProperty;
							rdfs:label	"hasDiagnosis";
							rdfs:domain	p4-lucat:LCPatient;
							rdfs:range	p4-lucat:Diagnosis;
							rdfs:comment ".";
							dcterms:modified "2018-11-27"^^xsd:date;
							dcterms:creator <https://www.tib.eu/en/research-development/scientific-data-management/staff/maria-isabel-castellanos/>.

p4-lucat:hasDiagnosis_imageBased     rdf:type     owl:ObjectProperty;
							rdfs:label	"hasDiagnosis_imageBased";
							rdfs:domain	p4-lucat:LCPatient;
							rdfs:range	p4-lucat:Diagnosis;
							rdfs:comment ".";
							dcterms:modified "2019-01-30"^^xsd:date;
							dcterms:creator <https://www.tib.eu/en/research-development/scientific-data-management/staff/samaneh-jozashoori/>.


p4-lucat:hasDiagnosisTumorStage   rdf:type     owl:ObjectProperty;
							rdfs:label	"hasDiagnosisTumorStage";
							rdfs:domain	p4-lucat:Diagnosis;
							rdfs:range	p4-lucat:TumorStage;
							rdfs:comment ".";
							dcterms:modified "2018-11-27"^^xsd:date;
							dcterms:creator <https://www.tib.eu/en/research-development/scientific-data-management/staff/maria-isabel-castellanos/>.

p4-lucat:hasDiagnosisTumorType   rdf:type     owl:ObjectProperty;
							rdfs:label	"hasDiagnosisTumorType";
							rdfs:domain	p4-lucat:Diagnosis;
							rdfs:range	p4-lucat:TumorType;
							rdfs:comment ".";
							dcterms:modified "2019-05-23"^^xsd:date;
							dcterms:creator <https://www.tib.eu/en/research-development/scientific-data-management/staff/maria-isabel-castellanos/>.

p4-lucat:hasDiagnosisPerformanceStatus   rdf:type     owl:ObjectProperty;
							rdfs:label	"hasDiagnosisPerformanceStatus";
							rdfs:domain	p4-lucat:Diagnosis;
							rdfs:range	p4-lucat:PerformanceStatus;
							rdfs:comment ".";
							dcterms:modified "2019-05-24"^^xsd:date;
							dcterms:creator <https://www.tib.eu/en/research-development/scientific-data-management/staff/maria-isabel-castellanos/>.

####### lc_similarity:
p4-lucat:isBetweenPatients	rdf:type        owl:ObjectProperty;	
				                rdfs:label	"isBetweenPatients";
						rdfs:domain	p4-lucat:PatientSimilarity;
						rdfs:range	p4-lucat:LCPatient;
						rdfs:comment	".";
						dcterms:modified "2018-11-27"^^xsd:date;
						dcterms:creator <https://www.tib.eu/en/research-development/scientific-data-management/staff/maria-isabel-castellanos/>.

################################### DatatypeProperties ###################################################
p4-lucat:briefSummary  rdf:type owl:DatatypeProperty;
                                        rdfs:subPropertyOf owl:topDataProperty;
                                        rdfs:domain p4-lucat:ClinicalTrial;
                                        rdfs:range xsd:string;
                                        rdfs:comment "This property shows the brief summary of clinical trials."@en;
                                        rdfs:isDefinedBy "emetis_niazmand"@en;
                                        rdfs:label "briefSummary"@en;
                                        owl:versionInfo "v1.0"@en.


p4-lucat:clinicalTrialId  rdf:type owl:DatatypeProperty;
                                           rdfs:subPropertyOf owl:topDataProperty;
                                           rdf:type owl:FunctionalProperty;
                                           rdfs:domain p4-lucat:ClinicalTrial;
                                           rdfs:range xsd:anyURI;
                                           rdfs:comment "This property shows the ids of clinical trials."@en;
                                           rdfs:isDefinedBy "emetis_niazmand"@en;
                                           rdfs:label "clinicalTrialId"@en;
                                           owl:versionInfo "v1.0"@en.



p4-lucat:clinicalTrialTitle  rdf:type owl:DatatypeProperty;
                                              rdfs:subPropertyOf owl:topDataProperty;
                                              rdfs:domain p4-lucat:ClinicalTrial;
                                              rdfs:range xsd:string;
                                              rdfs:comment "This property shows the titles of clinical trials."@en;
                                              rdfs:isDefinedBy "emetis_niazmand"@en;
                                              rdfs:label "clinicalTrialTitle"@en;
                                              owl:versionInfo "v1.0"@en.



p4-lucat:designAllocation rdf:type owl:DatatypeProperty;
                                            rdfs:subPropertyOf owl:topDataProperty;
                                            rdfs:domain p4-lucat:ClinicalTrial;
                                            rdfs:range xsd:anyURI;
                                            rdfs:comment "This property shows the allocation of design of clinical trials (e.g., Randomized or Non-Randomized)."@en;
                                            rdfs:isDefinedBy "emetis_niazmand"@en;
                                            rdfs:label "designAllocation"@en;
                                            owl:versionInfo "v1.0"@en.



p4-lucat:designPrimaryPurpose rdf:type owl:DatatypeProperty;
                                                rdfs:subPropertyOf owl:topDataProperty;
                                                rdfs:domain p4-lucat:ClinicalTrial;
                                                rdfs:range xsd:anyURI;
                                                rdfs:comment "This property shows the primary purpose (e.g., Treatment or Diagnostic)"@en;
                                                rdfs:isDefinedBy "emetis_niazmand"@en;
                                                rdfs:label "designPrimaryPurpose"@en;
                                                owl:versionInfo "v1.0"@en.



p4-lucat:detailedDescription rdf:type owl:DatatypeProperty;
                                               rdfs:subPropertyOf owl:topDataProperty;
                                               rdfs:domain p4-lucat:ClinicalTrial;
                                               rdfs:range xsd:string;
                                               rdfs:comment "This property shows the detailed description of clinical trials."@en;
                                               rdfs:isDefinedBy "emetis_niazmand"@en;
                                               rdfs:label "detailedDescription"@en;
                                               owl:versionInfo "v1.0"@en.


p4-lucat:maxAge    rdf:type 	  owl:DatatypeProperty;
                                  rdfs:subPropertyOf owl:topDataProperty;
                                  rdfs:domain p4-lucat:ClinicalTrial;
                                  rdfs:range xsd:string;
                                  rdfs:comment "This property shows the maximum age of patients or volunteers."@en;
                                  rdfs:isDefinedBy "emetis_niazmand"@en;
                                  rdfs:label "maxAge"@en;
                                  owl:versionInfo "v1.0"@en.



p4-lucat:minAge   rdf:type 	  owl:DatatypeProperty;
                                  rdfs:subPropertyOf owl:topDataProperty;
                                  rdf:type owl:FunctionalProperty;
                                  rdfs:domain p4-lucat:ClinicalTrial;
                                  rdfs:range xsd:string;
                                  rdfs:comment "This property shows the minimum age of patients or volunteers."@en;
                                  rdfs:isDefinedBy "emetis_niazmand"@en;
                                  rdfs:label "minAge"@en;
                                  owl:versionInfo "v1.0"@en.



p4-lucat:primaryOutTimeFrame rdf:type owl:DatatypeProperty;
                                               rdfs:subPropertyOf owl:topDataProperty;
                                               rdfs:domain p4-lucat:ClinicalTrial;
                                               rdfs:range xsd:string;
                                               rdfs:comment "This property shows the primary time frame (e.g., 18 months or 2 years)."@en;
                                               rdfs:isDefinedBy "emetis_niazmand"@en;
                                               rdfs:label "primaryOutTimeFrame"@en;
                                               owl:versionInfo "v1.0"@en.



p4-lucat:statusCT rdf:type owl:DatatypeProperty;
                                    rdfs:subPropertyOf owl:topDataProperty;
                                    rdf:type owl:FunctionalProperty;
                                    rdfs:domain p4-lucat:ClinicalTrial;
                                    rdfs:range xsd:anyURI;
                                    rdfs:comment "This property shows the overall status of clinical trials which are completed."@en;
                                    rdfs:isDefinedBy "emetis_niazmand"@en;
                                    rdfs:label "statusCT"@en;
                                    owl:versionInfo "v1.0"@en.
									
									
p4-lucat:annID	rdf:type	owl:DatatypeProperty;
			rdfs:label	"annID";
			rdfs:domain p4-lucat:Annotation;
			rdfs:range	rdfs:Literal;
			rdfs:comment	"Identification of instances of Annotation class";	
			dcterms:modified "2019-01-29"^^xsd:date;
			dcterms:creator <https://www.tib.eu/en/research-development/scientific-data-management/staff/samaneh-jozashoori/>.

p4-lucat:annLabel	rdf:type	owl:DatatypeProperty;
				rdfs:label	"annLabel";
				rdfs:domain	p4-lucat:Annotation;
				rdfs:range	rdfs:Literal;
                		rdfs:comment	"Label of instances of Annotation class";
				dcterms:modified "2018-04-12"^^xsd:date;
				dcterms:creator <https://www.tib.eu/en/research-development/scientific-data-management/staff/samaneh-jozashoori/>.

p4-lucat:annLabel_SPA	rdf:type	owl:DatatypeProperty;
				rdfs:label	"annLabel_SPA";
				rdfs:domain	p4-lucat:Annotation;
				rdfs:range	rdfs:Literal;
                		rdfs:comment	"Spanish label of instances of Annotation class";
				dcterms:modified "2019-01-30"^^xsd:date;
				dcterms:creator <https://www.tib.eu/en/research-development/scientific-data-management/staff/samaneh-jozashoori/>.

p4-lucat:semanticTypeID	rdf:type	owl:DatatypeProperty;
				rdfs:label	"semanticTypeID";
				rdfs:domain	p4-lucat:Annotation;
				rdfs:range	rdfs:Literal;
                rdfs:comment "The semantic type id provided by UMLS.";
				dcterms:modified "2019-01-30"^^xsd:date;
				dcterms:creator <https://www.tib.eu/en/research-development/scientific-data-management/staff/samaneh-jozashoori/>.

p4-lucat:semanticTypeLabel	rdf:type	owl:DatatypeProperty;
				rdfs:label	"semanticTypeLabel";
				rdfs:domain	p4-lucat:Annotation;
				rdfs:range	rdfs:Literal;
                rdfs:comment "The semantic type label provided by UMLS.";
				dcterms:modified "2020-10-05"^^xsd:date;
				dcterms:creator <https://www.tib.eu/en/research-development/scientific-data-management/staff/samaneh-jozashoori/>.

p4-lucat:semanticTypeGroup	rdf:type	owl:DatatypeProperty;
				rdfs:label	"semanticTypeGroup";
				rdfs:domain	p4-lucat:Annotation;
				rdfs:range	rdfs:Literal;
                rdfs:comment "The semantic type group provided by UMLS.";
				dcterms:modified "2020-10-05"^^xsd:date;
				dcterms:creator <https://www.tib.eu/en/research-development/scientific-data-management/staff/samaneh-jozashoori/>.								



#### WP4 requirements:

p4-lucat:pubmedID	rdf:type owl:DatatypeProperty;
					rdfs:label "PubMed ID";
					rdfs:domain p4-lucat:Publication;
				  	rdfs:range rdfs:Literal;
                  			rdfs:comment "PubMed ID.";
					dcterms:modified "2018-09-26"^^xsd:date;
					dcterms:creator <https://www.tib.eu/en/research-development/scientific-data-management/staff/samaneh-jozashoori/>.

p4-lucat:semanticType	rdf:type	owl:DatatypeProperty;
					rdfs:label	"semanticType";
					rdfs:domain	p4-lucat:Annotation;
					rdfs:range	rdfs:Literal;
					rdfs:comment	"A list with the allowed semantic_types for this Annotation in the UMLS. ";
					dcterms:modified "2018-11-27"^^xsd:date;
					dcterms:creator <https://www.tib.eu/en/research-development/scientific-data-management/staff/samaneh-jozashoori/>.

p4-lucat:year	rdf:type	owl:DatatypeProperty;
			rdfs:label	"year";
			rdfs:domain	p4-lucat:Publication;
			rdfs:range	rdfs:Literal;
			rdfs:comment	"Year of Publication";
			dcterms:modified "2018-04-12"^^xsd:date;
			dcterms:creator <https://www.tib.eu/en/research-development/scientific-data-management/staff/samaneh-jozashoori/>.


p4-lucat:authorName	rdf:type	owl:DatatypeProperty;
				rdfs:label	"authorName";
				rdfs:domain	p4-lucat:Author;
				rdfs:range	rdfs:Literal;
				rdfs:comment	"Name of Author";
				dcterms:modified "2019-05-24"^^xsd:date;
				dcterms:creator <https://www.tib.eu/en/research-development/scientific-data-management/staff/maria-isabel-castellanos/>.

p4-lucat:journal	rdf:type	owl:DatatypeProperty;
				rdfs:label	"journal";
				rdfs:domain	p4-lucat:Publication;
				rdfs:range	rdfs:Literal;
				rdfs:comment	"Journal of publication";
				dcterms:modified "2018-04-12"^^xsd:date;
				dcterms:creator <https://www.tib.eu/en/research-development/scientific-data-management/staff/samaneh-jozashoori/>. 

p4-lucat:rankingScore_SJR	rdf:type	owl:DatatypeProperty;
				rdfs:label	"rankingScore_SJR";
				rdfs:domain	p4-lucat:Publication;
				rdfs:range	rdfs:Literal;
				rdfs:comment	"ranking Score_SJR Journal of publication";
				dcterms:modified "2019-05-24"^^xsd:date;
				dcterms:creator <https://www.tib.eu/en/research-development/scientific-data-management/staff/maria-isabel-castellanos/>.

p4-lucat:rankingScore_hIndex	rdf:type	owl:DatatypeProperty;
				rdfs:label	"rankingScore_hIndex";
				rdfs:domain	p4-lucat:Publication;
				rdfs:range	rdfs:Literal;
				rdfs:comment	"ranking Score_hIndex of Journal of publication";
				dcterms:modified "2019-05-24"^^xsd:date;
				dcterms:creator <https://www.tib.eu/en/research-development/scientific-data-management/staff/maria-isabel-castellanos/>.


p4-lucat:publicationType	rdf:type	owl:DatatypeProperty;
				rdfs:label	"p4-lucat:publicationType";
				rdfs:domain	p4-lucat:Publication;
				rdfs:range	rdfs:Literal;
				rdfs:comment	"Type of Publication";
				dcterms:modified "2019-05-24"^^xsd:date;
				dcterms:creator <https://www.tib.eu/en/research-development/scientific-data-management/staff/maria-isabel-castellanos/>.

p4-lucat:authorAffiliation	rdf:type	owl:DatatypeProperty;
				rdfs:label	"authorAffiliation";
				rdfs:domain	p4-lucat:Publication;
				rdfs:range	rdfs:Literal;
				rdfs:comment	"Affiliation of Author";
				dcterms:modified "2019-05-24"^^xsd:date;
				dcterms:creator <https://www.tib.eu/en/research-development/scientific-data-management/staff/maria-isabel-castellanos/>.



p4-lucat:confidence     rdf:type     owl:DatatypeProperty;
							rdfs:label	"confidence";
							rdfs:domain	p4-lucat:Relation;
                                                      	rdfs:range	rdfs:Literal;
							rdfs:comment ".";
							dcterms:modified "2018-11-27"^^xsd:date;
							dcterms:creator <https://www.tib.eu/en/research-development/scientific-data-management/staff/maria-isabel-castellanos/>.

p4-lucat:negation     rdf:type     owl:DatatypeProperty;
							rdfs:label	"negation";
							rdfs:domain	p4-lucat:Relation;
                                                      	rdfs:range	rdfs:Literal;
							rdfs:comment ".";
							dcterms:modified "2019-05-24"^^xsd:date;
							dcterms:creator <https://www.tib.eu/en/research-development/scientific-data-management/staff/maria-isabel-castellanos/>.


p4-lucat:title     rdf:type     owl:DatatypeProperty;
							rdfs:label	"title";
							rdfs:domain	p4-lucat:Publication;
                                                      	rdfs:range	rdfs:Literal;
							rdfs:comment "Title of Publication.";
							dcterms:modified "2018-11-27"^^xsd:date;
							dcterms:creator <https://www.tib.eu/en/research-development/scientific-data-management/staff/maria-isabel-castellanos/>.


p4-lucat:publicationTypeName	rdf:type owl:DatatypeProperty;	
			                rdfs:label	"publicationTypeName";
							rdfs:domain	p4-lucat:PublicationType;
							rdfs:range	rdfs:Literal;
							rdfs:comment ".";
							dcterms:modified "2020-10-29"^^xsd:date;
							dcterms:creator <https://www.tib.eu/en/research-development/scientific-data-management/staff/samaneh-jozashoori/>.


p4-lucat:citedBy	rdf:type owl:DatatypeProperty;	
                rdfs:label	"citedBy";
				rdfs:domain	p4-lucat:Publication;
				rdfs:range	rdfs:Literal;
				rdfs:comment ".";
				dcterms:modified "2020-10-29"^^xsd:date;
				dcterms:creator <https://www.tib.eu/en/research-development/scientific-data-management/staff/samaneh-jozashoori/>.

p4-lucat:citedByLink	rdf:type owl:DatatypeProperty;	
	                rdfs:label	"citedByLink";
					rdfs:domain	p4-lucat:Publication;
					rdfs:range	rdfs:Literal;
					rdfs:comment ".";
					dcterms:modified "2020-10-29"^^xsd:date;
					dcterms:creator <https://www.tib.eu/en/research-development/scientific-data-management/staff/samaneh-jozashoori/>.

#### Drug requirements:

p4-lucat:drugLabel	rdf:type owl:DatatypeProperty;
					rdfs:label "DrugLabel";
					rdfs:domain p4-lucat:Drug;
				  	rdfs:range rdfs:Literal;
                  			rdfs:comment "Drug label.";
					dcterms:modified "2018-09-26"^^xsd:date;
					dcterms:creator <https://www.tib.eu/en/research-development/scientific-data-management/staff/samaneh-jozashoori/>.


p4-lucat:drugLabel_ENG	rdf:type owl:DatatypeProperty;
					rdfs:label "drugLabel_ENG";
					rdfs:domain p4-lucat:Drug;
				  	rdfs:range rdfs:Literal;
                  			rdfs:comment "Drug label.";
					dcterms:modified "2019-01-30"^^xsd:date;
					dcterms:creator <https://www.tib.eu/en/research-development/scientific-data-management/staff/samaneh-jozashoori/>.					

p4-lucat:disorderLabel_ENG	rdf:type owl:DatatypeProperty;
					rdfs:label "disorderLabel_ENG";
					rdfs:domain p4-lucat:Disorder;
				  	rdfs:range rdfs:Literal;
                  			rdfs:comment "Disorder label.";
					dcterms:modified "2019-05-24"^^xsd:date;
					dcterms:creator <https://www.tib.eu/en/research-development/scientific-data-management/staff/maria-isabel-castellanos/>.

p4-lucat:phenotypeLabel	rdf:type owl:DatatypeProperty;
					rdfs:label "PhenotypeLabel";
					rdfs:domain p4-lucat:Phenotype;
				  	rdfs:range rdfs:Literal;
                  			rdfs:comment "Phenotype Label.";
					dcterms:modified "2018-09-26"^^xsd:date;
					dcterms:creator <https://www.tib.eu/en/research-development/scientific-data-management/staff/samaneh-jozashoori/>.

p4-lucat:enzymeID	rdf:type owl:DatatypeProperty;
					rdfs:label "EnzymeID";
					rdfs:domain p4-lucat:Enzyme;
				  	rdfs:range rdfs:Literal;
                  			rdfs:comment "Enzyme ID.";
					dcterms:modified "2018-09-26"^^xsd:date;
					dcterms:creator <https://www.tib.eu/en/research-development/scientific-data-management/staff/samaneh-jozashoori/>.

p4-lucat:enzymeLabel	rdf:type owl:DatatypeProperty;
					rdfs:label "EnzymeLabel";
					rdfs:domain p4-lucat:Enzyme;
				  	rdfs:range rdfs:Literal;
                  			rdfs:comment "Enzyme Label.";
					dcterms:modified "2018-09-26"^^xsd:date;
					dcterms:creator <https://www.tib.eu/en/research-development/scientific-data-management/staff/samaneh-jozashoori/>.


p4-lucat:dse_AvgFrequency	rdf:type	owl:DatatypeProperty;
						rdfs:label	"dse_AvgFrequency";
						rdfs:domain	p4-lucat:DrugSideEffect;
						rdfs:range	rdfs:Literal;
						rdfs:comment	"Represents the average frequecy of particular drug having specific side effect.";
						dcterms:modified "2018-07-24"^^xsd:date;
						dcterms:creator <https://www.tib.eu/en/research-development/scientific-data-management/staff/samaneh-jozashoori/>.

p4-lucat:externalLink	rdf:type owl:DatatypeProperty;
					rdfs:label "externalLink";
					rdfs:domain p4-lucat:Concept;
				  	rdfs:range xsd:anyURI;
                  	rdfs:comment "Link to external resources.";
					dcterms:modified "2018-09-26"^^xsd:date;
					dcterms:creator <https://www.tib.eu/en/research-development/scientific-data-management/staff/samaneh-jozashoori/>.


p4-lucat:targetID	rdf:type owl:DatatypeProperty;
					rdfs:label "targetID";
					rdfs:domain p4-lucat:Target;
				  	rdfs:range rdfs:Literal;
                  			rdfs:comment "Target ID.";
					dcterms:modified "2018-10-30"^^xsd:date;
					dcterms:creator <https://www.tib.eu/en/research-development/scientific-data-management/staff/samaneh-jozashoori/>.

p4-lucat:targetLabel	rdf:type owl:DatatypeProperty;
					rdfs:label "TargetLabel";
					rdfs:domain p4-lucat:Target;
				  	rdfs:range rdfs:Literal;
                  			rdfs:comment "Target Label.";
					dcterms:modified "2018-10-30"^^xsd:date;
					dcterms:creator <https://www.tib.eu/en/research-development/scientific-data-management/staff/samaneh-jozashoori/>.

p4-lucat:proteinID	rdf:type owl:DatatypeProperty;
					rdfs:label "proteinID";
					rdfs:domain p4-lucat:Protein;
				  	rdfs:range rdfs:Literal;
                  			rdfs:comment "Protein ID.";
					dcterms:modified "2020-07-24"^^xsd:date;
					dcterms:creator <https://www.tib.eu/en/research-development/scientific-data-management/staff/samaneh-jozashoori/>.

p4-lucat:proteinLabel	rdf:type owl:DatatypeProperty;
					rdfs:label "proteinName";
					rdfs:domain p4-lucat:Protein;
				  	rdfs:range rdfs:Literal;
                  			rdfs:comment "Protein Label.";
					dcterms:modified "2020-07-24"^^xsd:date;
					dcterms:creator <https://www.tib.eu/en/research-development/scientific-data-management/staff/samaneh-jozashoori/>.


p4-lucat:uniprotID	rdf:type owl:DatatypeProperty;
					rdfs:label "uniprotID";
					rdfs:domain p4-lucat:Concept;
				  	rdfs:range rdfs:Literal;
                  			rdfs:comment "External connection to accession ID in uniprot.";
					dcterms:modified "2018-10-30"^^xsd:date;
					dcterms:creator <https://www.tib.eu/en/research-development/scientific-data-management/staff/samaneh-jozashoori/>.

p4-lucat:disorderLabel	rdf:type owl:DatatypeProperty;
					rdfs:label "DisorderLabel";
					rdfs:domain p4-lucat:Disorder;
				  	rdfs:range rdfs:Literal;
                  			rdfs:comment "Disorder Label.";
					dcterms:modified "2018-10-30"^^xsd:date;
					dcterms:creator <https://www.tib.eu/en/research-development/scientific-data-management/staff/samaneh-jozashoori/>.

p4-lucat:disorderLabel_SPA 	rdf:type owl:DatatypeProperty;
					rdfs:label "disorderLabel_SPA";
					rdfs:domain p4-lucat:Disorder;
				  	rdfs:range rdfs:Literal;
                  			rdfs:comment "Disorder Label_SPA.";
					dcterms:modified "2018-11-25"^^xsd:date;
					dcterms:creator <https://www.tib.eu/en/research-development/scientific-data-management/staff/maria-isabel-castellanos/>.


p4-lucat:impact	rdf:type	owl:DatatypeProperty;
						rdfs:lasbel	"impact";
						rdfs:domain	p4-lucat:AdverseEvent;
						rdfs:range	rdfs:Literal;
						rdfs:comment	"Represents the type impact of the adverse event i.e. increase/decrease";
						dcterms:modified "2020-09-14"^^xsd:date;
						dcterms:creator <https://www.tib.eu/en/research-development/scientific-data-management/staff/samaneh-jozashoori/>.			


p4-lucat:toxicityType	rdf:type	owl:DatatypeProperty;
							rdfs:label	"toxicityType";
							rdfs:domain	p4-lucat:Phenotype;
							rdfs:range	rdfs:Literal;
							rdfs:comment	"An attribute of phenotype represetning the type of the toxicity.";
							dcterms:modified "2020-07-24"^^xsd:date;
							dcterms:creator <https://www.tib.eu/en/research-development/scientific-data-management/staff/samaneh-jozashoori/>.	


p4-lucat:predictionMethod	rdf:type	owl:DatatypeProperty;
							rdfs:label	"predictionMethod";
							rdfs:domain	p4-lucat:Interaction;
							rdfs:range	rdfs:Literal;
							rdfs:comment "Represents the prediction method that is used in order to extract DDI predictions from literature or databases.";
							dcterms:modified "2020-10-29"^^xsd:date;
							dcterms:creator <https://www.tib.eu/en/research-development/scientific-data-management/staff/samaneh-jozashoori/>.	

p4-lucat:methodAbbreviation	rdf:type	owl:DatatypeProperty;
							rdfs:label	"methodAbbreviation";
							rdfs:domain	p4-lucat:Interaction;
							rdfs:range	rdfs:Literal;
							rdfs:comment "Represents the abbreviation of the prediction method that is used.";
							dcterms:modified "2020-10-29"^^xsd:date;
							dcterms:creator <https://www.tib.eu/en/research-development/scientific-data-management/staff/samaneh-jozashoori/>.	


#### WP2 requirements:
##### lc_notes:


p4-lucat:familiarAntecedentLabel_ENG	rdf:type        owl:DatatypeProperty;	
				rdfs:label	"familiarAntecedentLabel_ENG";
						rdfs:domain	p4-lucat:FamiliarAntecedent;
						rdfs:range	rdfs:Literal;
						rdfs:comment	"The title of familiar antecedent.";
						dcterms:modified "2018-11-27"^^xsd:date;
						dcterms:creator <https://www.tib.eu/en/research-development/scientific-data-management/staff/maria-isabel-castellanos/>.


p4-lucat:hasDate 	rdf:type owl:DatatypeProperty;	
				rdfs:label	"hasDate";
				rdfs:domain	p4-lucat:Concept;
				rdfs:range	rdfs:Literal;
				rdfs:comment "Connection between any concept and the corresponding date.";
				dcterms:modified "2021-03-18"^^xsd:date;
				dcterms:creator <https://www.tib.eu/en/research-development/scientific-data-management/staff/samaneh-jozashoori/>.


p4-lucat:biomarkerLabel	rdf:type	owl:DatatypeProperty;
				rdfs:label	"biomarkerLabel";
				rdfs:domain	p4-lucat:Biomarker;
				rdfs:range	rdfs:Literal;
				rdfs:comment	"The name of biomarker.";
				dcterms:modified "2018-11-22"^^xsd:date;
				dcterms:creator   <https://www.tib.eu/en/research-development/scientific-data-management/staff/maria-isabel-castellanos/>.

p4-lucat:survivalMonths	rdf:type	owl:DatatypeProperty;
				rdfs:label	"survivalMonths";
				rdfs:domain	p4-lucat:LCPatient;
				rdfs:range	rdfs:Literal;
				rdfs:comment	"Months from diagnosis to death or until the last documented record of the patient.";
				dcterms:modified "2017-10-04"^^xsd:date;
				dcterms:creator <https://www.tib.eu/en/research-development/scientific-data-management/staff/samaneh-jozashoori/>.

p4-lucat:sampleDate	rdf:type	owl:DatatypeProperty;
					rdfs:label	"sampleDate";
					rdfs:domain	p4-lucat:LiquidBiopsy;
					rdfs:range	rdfs:Literal;
					rdfs:comment "Date on which the biopsy sample has been taken.";
					dcterms:modified "2021-03-18"^^xsd:date;
					dcterms:creator <https://www.tib.eu/en/research-development/scientific-data-management/staff/samaneh-jozashoori/>.

p4-lucat:resultDate	rdf:type	owl:DatatypeProperty;
					rdfs:label	"resultDate";
					rdfs:domain	p4-lucat:LiquidBiopsy;
					rdfs:range	rdfs:Literal;
					rdfs:comment "Date on which the biopsy result has been provided.";
					dcterms:modified "2021-03-18"^^xsd:date;
					dcterms:creator <https://www.tib.eu/en/research-development/scientific-data-management/staff/samaneh-jozashoori/>.

p4-lucat:targetTotal	rdf:type	owl:DatatypeProperty;
					rdfs:label	"targetTotal";
					rdfs:domain	p4-lucat:LiquidBiopsy;
					rdfs:range	rdfs:Literal;
					rdfs:comment "The percentage of circulating tumor DNA in the blood";
					dcterms:modified "2017-07-24"^^xsd:date;
					dcterms:creator <https://www.tib.eu/en/research-development/scientific-data-management/staff/samaneh-jozashoori/>.

p4-lucat:copiesMicroliterFam	rdf:type	owl:DatatypeProperty;
							rdfs:label	"copiesMicroliterFam";
							rdfs:domain	p4-lucat:LiquidBiopsy;
							rdfs:range	rdfs:Literal;
							rdfs:comment "Number of mutated copies per microliter of blood";
							dcterms:modified "2017-07-24"^^xsd:date;
							dcterms:creator <https://www.tib.eu/en/research-development/scientific-data-management/staff/samaneh-jozashoori/>.

p4-lucat:copiesMicroliterVic	rdf:type	owl:DatatypeProperty;
							rdfs:label	"copiesMicroliterVic";
							rdfs:domain	p4-lucat:LiquidBiopsy;
							rdfs:range	rdfs:Literal;
							rdfs:comment "Number of non-mutated copies per microliter of blood";
							dcterms:modified "2017-07-24"^^xsd:date;
							dcterms:creator <https://www.tib.eu/en/research-development/scientific-data-management/staff/samaneh-jozashoori/>.

p4-lucat:tumorTypeLabel_ENG	rdf:type owl:DatatypeProperty;
					rdfs:label "tumorTypeLabel_ENG";
					rdfs:domain p4-lucat:TumorType;
				  	rdfs:range rdfs:Literal;
                  			rdfs:comment "English tumor Type Label.";
					dcterms:modified "2018-11-27"^^xsd:date;
					dcterms:creator <https://www.tib.eu/en/research-development/scientific-data-management/staff/maria-isabel-castellanos/>.

p4-lucat:secondTumorTypeLabel	rdf:type owl:DatatypeProperty;
					rdfs:label "secondTumorTypeLabel";
					rdfs:domain p4-lucat:TumorType;
				  	rdfs:range rdfs:Literal;
                  			rdfs:comment "second tumor Type Label.";
					dcterms:modified "2019-05-24"^^xsd:date;
					dcterms:creator <https://www.tib.eu/en/research-development/scientific-data-management/staff/maria-isabel-castellanos/>.


p4-lucat:drugLabel_SPA	 rdf:type  owl:DatatypeProperty;
					rdfs:label "drugLabel_SPA";	
                                        rdfs:domain p4-lucat:Drug;
               			        rdfs:range rdfs:Literal;
					rdfs:comment	"";
					dcterms:modified "2018-11-26"^^xsd:date;
					dcterms:creator <https://www.tib.eu/en/research-development/scientific-data-management/staff/maria-isabel-castellanos/>.

p4-lucat:drugBankID rdf:type owl:DatatypeProperty;
					rdfs:label "DrugBankID";
					rdfs:domain p4-lucat:Drug;
				  	rdfs:range rdfs:Literal;
                  			rdfs:comment "Drug Bank ID.";
					dcterms:modified "2018-11-22"^^xsd:date;
					dcterms:creator <https://www.tib.eu/en/research-development/scientific-data-management/staff/maria-isabel-castellanos/>.

p4-lucat:drugGroupLabel  rdf:type owl:DatatypeProperty;
					rdfs:label "drugGroupLabel";
					rdfs:domain p4-lucat:DrugGroup;
				  	rdfs:range rdfs:Literal;
                  			rdfs:comment "Drug Group Label.";
					dcterms:modified "2018-11-26"^^xsd:date;
					dcterms:creator <https://www.tib.eu/en/research-development/scientific-data-management/staff/maria-isabel-castellanos/>.

p4-lucat:drugGroupLabel_SPA  rdf:type owl:DatatypeProperty;
					rdfs:label "drugGroupLabel_SPA";
					rdfs:domain p4-lucat:DrugGroup;
				  	rdfs:range rdfs:Literal;
                  			rdfs:comment "Drug Group Label_SPA.";
					dcterms:modified "2018-11-26"^^xsd:date;
					dcterms:creator <https://www.tib.eu/en/research-development/scientific-data-management/staff/maria-isabel-castellanos/>.


p4-lucat:tumorStageLabel      rdf:type     owl:DatatypeProperty;
							rdfs:label	"tumorStageLabel";
							rdfs:domain	p4-lucat:TumorStage;
							rdfs:range	rdfs:Literal;
							rdfs:comment ".";
							dcterms:modified "2018-11-27"^^xsd:date;
							dcterms:creator <https://www.tib.eu/en/research-development/scientific-data-management/staff/maria-isabel-castellanos/>.


p4-lucat:toxicityLabel_ENG 	rdf:type        owl:DatatypeProperty;	
				rdfs:label	"toxicityLabel_ENG";
						rdfs:domain	p4-lucat:Phenotype;
						rdfs:range	rdfs:Literal;
						rdfs:comment	".";
						dcterms:modified "2019-05-24"^^xsd:date;
						dcterms:creator  <https://www.tib.eu/en/research-development/scientific-data-management/staff/maria-isabel-castellanos/>.

p4-lucat:distanceToHospital	rdf:type        owl:DatatypeProperty;	
				        rdfs:label	"distanceToHospital";
						rdfs:domain	p4-lucat:LCPatient;
						rdfs:range	rdfs:Literal;
						rdfs:comment "Represents the distance in kilometers from the city in which the patient lives to the hospital.";
						dcterms:modified "2020-07-21"^^xsd:date;
						dcterms:creator <https://www.tib.eu/en/research-development/scientific-data-management/staff/samaneh-jozashoori/>.		

p4-lucat:beingIn_hospitalHealthArea	rdf:type        owl:DatatypeProperty;	
				        rdfs:label	"beingIn_hospitalHealthArea";
						rdfs:domain	p4-lucat:LCPatient;
						rdfs:range	rdfs:Literal;
						rdfs:comment "Represents if the patient lives in a city which belong to the municipal scope area awarded to the hospital. Format: Boolean";
						dcterms:modified "2020-07-21"^^xsd:date;
						dcterms:creator <https://www.tib.eu/en/research-development/scientific-data-management/staff/samaneh-jozashoori/>.	

p4-lucat:existenceOf_brainMetastasis	rdf:type        owl:DatatypeProperty;	
				        rdfs:label	"existenceOf_brainMetastasis";
						rdfs:domain	p4-lucat:LCPatient;
						rdfs:range	rdfs:Literal;
						rdfs:comment "Represents if brain metastasis has been detected in Entity. Format: Boolean";
						dcterms:modified "2020-07-21"^^xsd:date;
						dcterms:creator <https://www.tib.eu/en/research-development/scientific-data-management/staff/samaneh-jozashoori/>.	

p4-lucat:existenceOf_bioRos1	rdf:type        owl:DatatypeProperty;	
				        rdfs:label	"existenceOf_bioRos1";
						rdfs:domain	p4-lucat:LCPatient;
						rdfs:range	rdfs:Literal;
						rdfs:comment "Represents the aggregated results of the biopsies performed to the Entity for the particular biomarker called ROS1. In particular, represents if an Entity has been studied, and if the result has been positive or negative in this specific biomarker. Format: Boolean";
						dcterms:modified "2020-07-21"^^xsd:date;
						dcterms:creator <https://www.tib.eu/en/research-development/scientific-data-management/staff/samaneh-jozashoori/>.

p4-lucat:existenceOf_bioEgfr	rdf:type        owl:DatatypeProperty;	
				        rdfs:label	"existenceOf_bioEgfr";
						rdfs:domain	p4-lucat:LCPatient;
						rdfs:range	rdfs:Literal;
						rdfs:comment "Meaning: Represents the aggregated results of the biopsies performed to the Entity for the particular biomarker called EGFR. In particular, represents if an Entity has been studied, and if the result has been positive or negative in this specific biomarker. Format: Boolean";
						dcterms:modified "2020-07-21"^^xsd:date;
						dcterms:creator <https://www.tib.eu/en/research-development/scientific-data-management/staff/samaneh-jozashoori/>.	

p4-lucat:existenceOf_bioAlk	rdf:type        owl:DatatypeProperty;	
				        rdfs:label	"existenceOf_bioAlk";
						rdfs:domain	p4-lucat:LCPatient;
						rdfs:range	rdfs:Literal;
						rdfs:comment "Meaning: Represents the aggregated results of the biopsies performed to the Entity for the particular biomarker called ALK. In particular, represents if an Entity has been studied, and if the result has been positive or negative in this specific biomarker. Format: Boolean";
						dcterms:modified "2020-07-21"^^xsd:date;
						dcterms:creator <https://www.tib.eu/en/research-development/scientific-data-management/staff/samaneh-jozashoori/>.	

p4-lucat:existenceOf_biomarker	rdf:type        owl:DatatypeProperty;	
				        rdfs:label	"existenceOf_biomarker";
						rdfs:domain	p4-lucat:LCPatient;
						rdfs:range	rdfs:Literal;
						rdfs:comment "Meaning: Represents the aggregated results of the biopsies of any biomarker performed to the Entity. In particular, represents if an Entity has been studied, and if the result has been positive or negative in any biomarker.";
						dcterms:modified "2020-07-21"^^xsd:date;
						dcterms:creator <https://www.tib.eu/en/research-development/scientific-data-management/staff/samaneh-jozashoori/>.	

p4-lucat:existenceOf_tki	rdf:type        owl:DatatypeProperty;	
				        rdfs:label	"existenceOf_tki";
						rdfs:domain	p4-lucat:LCPatient;
						rdfs:range	rdfs:Literal;
						rdfs:comment "Represents if Entity has received tki oncology treatment. Format: Boolean";
						dcterms:modified "2020-07-21"^^xsd:date;
						dcterms:creator <https://www.tib.eu/en/research-development/scientific-data-management/staff/samaneh-jozashoori/>.	

p4-lucat:smoking	rdf:type        owl:DatatypeProperty;	
				        rdfs:label	"smoking";
						rdfs:domain	p4-lucat:LCPatient;
						rdfs:range	rdfs:Literal;
						rdfs:comment "Represents if current of former smoker the number of cigarettes per year.";
						dcterms:modified "2020-07-21"^^xsd:date;
						dcterms:creator <https://www.tib.eu/en/research-development/scientific-data-management/staff/samaneh-jozashoori/>.	

p4-lucat:placeOfDeath	rdf:type        owl:DatatypeProperty;	
				        rdfs:label	"placeOfDeath";
						rdfs:domain	p4-lucat:LCPatient;
						rdfs:range	rdfs:Literal;
						rdfs:comment "Represents the location where the patient died [home, hospital]; value [alive] is returned if patients has not died.";
						dcterms:modified "2020-07-21"^^xsd:date;
						dcterms:creator <https://www.tib.eu/en/research-development/scientific-data-management/staff/samaneh-jozashoori/>.	

p4-lucat:existenceOf_familiarAntecedents	rdf:type        owl:DatatypeProperty;	
				        rdfs:label	"existenceOf_familiarAntecedents";
						rdfs:domain	p4-lucat:LCPatient;
						rdfs:range	rdfs:Literal;
						rdfs:comment "Represents if the Entity has familiars with antecedents of cancer. Format: Boolean";
						dcterms:modified "2020-07-21"^^xsd:date;
						dcterms:creator <https://www.tib.eu/en/research-development/scientific-data-management/staff/samaneh-jozashoori/>.	

p4-lucat:existenceOf_radiationtherapy	rdf:type        owl:DatatypeProperty;	
				        rdfs:label	"existenceOf_radiationtherapy";
						rdfs:domain	p4-lucat:LCPatient;
						rdfs:range	rdfs:Literal;
						rdfs:comment "If Entity has received radiationtherapy oncology treatment. Format: Boolean";
						dcterms:modified "2020-07-21"^^xsd:date;
						dcterms:creator <https://www.tib.eu/en/research-development/scientific-data-management/staff/samaneh-jozashoori/>.	

p4-lucat:ageAtDeath	rdf:type        owl:DatatypeProperty;	
				        rdfs:label	"ageAtDeath";
						rdfs:domain	p4-lucat:LCPatient;
						rdfs:range	rdfs:Literal;
						rdfs:comment "Represents the age when the patient dead.";
						dcterms:modified "2020-07-21"^^xsd:date;
						dcterms:creator <https://www.tib.eu/en/research-development/scientific-data-management/staff/samaneh-jozashoori/>.	

p4-lucat:isDead	rdf:type        owl:DatatypeProperty;	
				        rdfs:label	"isDead";
						rdfs:domain	p4-lucat:LCPatient;
						rdfs:range	rdfs:Literal;
						rdfs:comment "Represents if the patient is currently dead. Format: Boolean";
						dcterms:modified "2020-07-21"^^xsd:date;
						dcterms:creator <https://www.tib.eu/en/research-development/scientific-data-management/staff/samaneh-jozashoori/>.	

p4-lucat:existenceOf_chemotherapy	rdf:type        owl:DatatypeProperty;	
				        rdfs:label	"existenceOf_chemotherapy";
						rdfs:domain	p4-lucat:LCPatient;
						rdfs:range	rdfs:Literal;
						rdfs:comment "Represents if Entity has received chemotherapy oncology treatment. Format: Boolean";
						dcterms:modified "2020-07-21"^^xsd:date;
						dcterms:creator <https://www.tib.eu/en/research-development/scientific-data-management/staff/samaneh-jozashoori/>.	

p4-lucat:existenceOf_surgery	rdf:type        owl:DatatypeProperty;	
				        rdfs:label	"existenceOf_surgery";
						rdfs:domain	p4-lucat:LCPatient;
						rdfs:range	rdfs:Literal;
						rdfs:comment "Represents whether a surgery has been performed to an Entity. Format: Boolean";
						dcterms:modified "2020-07-21"^^xsd:date;
						dcterms:creator <https://www.tib.eu/en/research-development/scientific-data-management/staff/samaneh-jozashoori/>.	

p4-lucat:numberOfCigarettesPerYear	rdf:type        owl:DatatypeProperty;	
				        rdfs:label	"numberOfCigarettesPerYear";
						rdfs:domain	p4-lucat:LCPatient;
						rdfs:range	rdfs:Literal;
						rdfs:comment "Represents if current of former smoker the number of cigarettes per year.";
						dcterms:modified "2020-07-21"^^xsd:date;
						dcterms:creator <https://www.tib.eu/en/research-development/scientific-data-management/staff/samaneh-jozashoori/>.	

p4-lucat:existenceOf_antiangiogentic	rdf:type        owl:DatatypeProperty;	
				        rdfs:label	"existenceOf_antiangiogentic";
						rdfs:domain	p4-lucat:LCPatient;
						rdfs:range	rdfs:Literal;
						rdfs:comment "If Entity has received antiangiogenic oncology treatment. Format: Boolean";
						dcterms:modified "2020-07-21"^^xsd:date;
						dcterms:creator <https://www.tib.eu/en/research-development/scientific-data-management/staff/samaneh-jozashoori/>.	

p4-lucat:existenceOf_immunotherapy	rdf:type        owl:DatatypeProperty;	
				        rdfs:label	"existenceOf_immunotherapy";
						rdfs:domain	p4-lucat:LCPatient;
						rdfs:range	rdfs:Literal;
						rdfs:comment "If Entity has received immunotherapy oncology treatment. Format: Boolean";
						dcterms:modified "2020-07-21"^^xsd:date;
						dcterms:creator <https://www.tib.eu/en/research-development/scientific-data-management/staff/samaneh-jozashoori/>.																																																																																												


p4-lucat:existenceOf_cutaneaToxicity	rdf:type        owl:DatatypeProperty;	
				        rdfs:label	"existenceOf_cutaneaToxicity";
						rdfs:domain	p4-lucat:OncologicalTreatmentLine;
						rdfs:range	rdfs:Literal;
						rdfs:comment "if the patient developed any toxicity of kind cutanea during the line. Format: Boolean.";
						dcterms:modified "2020-07-21"^^xsd:date;
						dcterms:creator <https://www.tib.eu/en/research-development/scientific-data-management/staff/samaneh-jozashoori/>.	

p4-lucat:existenceOf_toxicity	rdf:type        owl:DatatypeProperty;	
				        rdfs:label	"existenceOf_toxicity";
						rdfs:domain	p4-lucat:OncologicalTreatmentLine;
						rdfs:range	rdfs:Literal;
						rdfs:comment "if the patient developed any toxicity. Format: Boolean.";
						dcterms:modified "2020-07-21"^^xsd:date;
						dcterms:creator <https://www.tib.eu/en/research-development/scientific-data-management/staff/samaneh-jozashoori/>.	

p4-lucat:treatmentLineNumber	rdf:type        owl:DatatypeProperty;	
					        rdfs:label	"treatmentLineNumber";
							rdfs:domain	p4-lucat:OncologicalTreatmentLine;
							rdfs:range	rdfs:Literal;
							rdfs:comment "Line of treatment number.";
							dcterms:modified "2020-07-21"^^xsd:date;
							dcterms:creator <https://www.tib.eu/en/research-development/scientific-data-management/staff/samaneh-jozashoori/>.	

p4-lucat:treatmentDurationMonths	rdf:type        owl:DatatypeProperty;	
				        rdfs:label	"treatmentDurationMonths";
						rdfs:domain	p4-lucat:OncologicalTreatmentLine;
						rdfs:range	rdfs:Literal;
						rdfs:comment "The duration of the line of treatment in months";
						dcterms:modified "2020-07-21"^^xsd:date;
						dcterms:creator <https://www.tib.eu/en/research-development/scientific-data-management/staff/samaneh-jozashoori/>.	

p4-lucat:existenceOf_neurologicalToxicity	rdf:type        owl:DatatypeProperty;	
				        rdfs:label	"existenceOf_neurologicalToxicity";
						rdfs:domain	p4-lucat:OncologicalTreatmentLine;
						rdfs:range	rdfs:Literal;
						rdfs:comment "if the patient developed any toxicity of kind neurological during the line. Format: Boolean.";
						dcterms:modified "2020-07-21"^^xsd:date;
						dcterms:creator <https://www.tib.eu/en/research-development/scientific-data-management/staff/samaneh-jozashoori/>.	

p4-lucat:existenceOf_gastrointestinalToxicity	rdf:type        owl:DatatypeProperty;	
				        rdfs:label	"existenceOf_gastrointestinalToxicity";
						rdfs:domain	p4-lucat:OncologicalTreatmentLine;
						rdfs:range	rdfs:Literal;
						rdfs:comment "if the patient developed any toxicity of kind gastrointestinal during the line. Format: Boolean.";
						dcterms:modified "2020-07-21"^^xsd:date;
						dcterms:creator <https://www.tib.eu/en/research-development/scientific-data-management/staff/samaneh-jozashoori/>.	

p4-lucat:existenceOf_generalToxicity	rdf:type        owl:DatatypeProperty;	
				        rdfs:label	"existenceOf_generalToxicity";
						rdfs:domain	p4-lucat:OncologicalTreatmentLine;
						rdfs:range	rdfs:Literal;
						rdfs:comment "if the patient developed any toxicity of kind general during the line. Format: Boolean.";
						dcterms:modified "2020-07-21"^^xsd:date;
						dcterms:creator <https://www.tib.eu/en/research-development/scientific-data-management/staff/samaneh-jozashoori/>.	

p4-lucat:existenceOf_neumologicalToxicity	rdf:type        owl:DatatypeProperty;	
				        rdfs:label	"existenceOf_neumologicalToxicity";
						rdfs:domain	p4-lucat:OncologicalTreatmentLine;
						rdfs:range	rdfs:Literal;
						rdfs:comment "if the patient developed any toxicity of kind neumological during the line. Format: Boolean.";
						dcterms:modified "2020-07-21"^^xsd:date;
						dcterms:creator <https://www.tib.eu/en/research-development/scientific-data-management/staff/samaneh-jozashoori/>.	

p4-lucat:existenceOf_analyticalToxicity	rdf:type        owl:DatatypeProperty;	
				        rdfs:label	"existenceOf_gastrointestinalToxicity";
						rdfs:domain	p4-lucat:existenceOf_analyticalToxicity;
						rdfs:range	rdfs:Literal;
						rdfs:comment "if the patient developed any toxicity of kind analytical during the line. Format: Boolean.";
						dcterms:modified "2020-07-21"^^xsd:date;
						dcterms:creator <https://www.tib.eu/en/research-development/scientific-data-management/staff/samaneh-jozashoori/>.	

p4-lucat:existenceOf_otherToxicity	rdf:type        owl:DatatypeProperty;	
				        rdfs:label	"existenceOf_otherToxicity";
						rdfs:domain	p4-lucat:OncologicalTreatmentLine;
						rdfs:range	rdfs:Literal;
						rdfs:comment "if the patient developed any toxicity of kind other during the line. Format: Boolean.";
						dcterms:modified "2020-07-21"^^xsd:date;
						dcterms:creator <https://www.tib.eu/en/research-development/scientific-data-management/staff/samaneh-jozashoori/>.	

p4-lucat:existenceOf_endocrinaToxicity	rdf:type        owl:DatatypeProperty;	
				        rdfs:label	"existenceOf_endocrinaToxicity";
						rdfs:domain	p4-lucat:OncologicalTreatmentLine;
						rdfs:range	rdfs:Literal;
						rdfs:comment "if the patient developed any toxicity of kind endocrina during the line. Format: Boolean.";
						dcterms:modified "2020-07-22"^^xsd:date;
						dcterms:creator <https://www.tib.eu/en/research-development/scientific-data-management/staff/samaneh-jozashoori/>.	

p4-lucat:existenceOf_brainMetastasis	rdf:type        owl:DatatypeProperty;	
				        rdfs:label	"existenceOf_brainMetastasis";
						rdfs:domain	p4-lucat:OncologicalTreatmentLine;
						rdfs:range	rdfs:Literal;
						rdfs:comment "Represents if brain metastasis has been detected in Entity. Format: Boolean.";
						dcterms:modified "2020-07-22"^^xsd:date;
						dcterms:creator <https://www.tib.eu/en/research-development/scientific-data-management/staff/samaneh-jozashoori/>.	

p4-lucat:treatmentType	rdf:type        owl:DatatypeProperty;	
				        rdfs:label	"treatmentType";
						rdfs:domain	p4-lucat:OncologicalTreatmentLine;
						rdfs:range	rdfs:Literal;
						rdfs:comment "An attribute of oncological treatment line representing the treatment type.";
						dcterms:modified "2020-07-22"^^xsd:date;
						dcterms:creator <https://www.tib.eu/en/research-development/scientific-data-management/staff/samaneh-jozashoori/>.	

p4-lucat:treatmentFinishDate	rdf:type        owl:DatatypeProperty;	
				        rdfs:label	"treatmentFinishDate";
						rdfs:domain	p4-lucat:OncologicalTreatmentLine;
						rdfs:range	rdfs:Literal;
						rdfs:comment "Relation between the treatment line and the finishing date of the treatment line.";
						dcterms:modified "2021-03-18"^^xsd:date;
						dcterms:creator <https://www.tib.eu/en/research-development/scientific-data-management/staff/samaneh-jozashoori/>.	

p4-lucat:treatmentInitDate	rdf:type        owl:DatatypeProperty;	
				        rdfs:label	"treatmentInitDate";
						rdfs:domain	p4-lucat:OncologicalTreatmentLine;
						rdfs:range	rdfs:Literal;
						rdfs:comment "Relation between the treatment line and the initiation date of the treatment line.";
						dcterms:modified "2021-03-18"^^xsd:date;
						dcterms:creator <https://www.tib.eu/en/research-development/scientific-data-management/staff/samaneh-jozashoori/>.																																																							


p4-lucat:oncologicalSurgeryLabel_ENG	rdf:type        owl:DatatypeProperty;	
				        rdfs:label	"oncologicalSurgeryLabel_ENG";
						rdfs:domain	p4-lucat:OncologicalSurgery;
						rdfs:range	rdfs:Literal;
						rdfs:comment "Represents English label of the oncological surgery value.";
						dcterms:modified "2020-07-21"^^xsd:date;
						dcterms:creator <https://www.tib.eu/en/research-development/scientific-data-management/staff/samaneh-jozashoori/>.	


p4-lucat:hasDurationInHospital	rdf:type        owl:DatatypeProperty;	
				        rdfs:label	"hasDurationInHospital";
						rdfs:domain	p4-lucat:HospitalProcess;
						rdfs:range	rdfs:Literal;
						rdfs:comment "An attribute of the service reason representing the duration of the hospital process in days.";
						dcterms:modified "2020-07-21"^^xsd:date;
						dcterms:creator <https://www.tib.eu/en/research-development/scientific-data-management/staff/samaneh-jozashoori/>.	

p4-lucat:hasProcessId	rdf:type        owl:DatatypeProperty;	
				        rdfs:label	"hasProcessId";
						rdfs:domain	p4-lucat:HospitalProcess;
						rdfs:range	rdfs:Literal;
						rdfs:comment "Relation between the hospital process and the unique identifier of the it.";
						dcterms:modified "2020-07-21"^^xsd:date;
						dcterms:creator <https://www.tib.eu/en/research-development/scientific-data-management/staff/samaneh-jozashoori/>.		

p4-lucat:hasGeneratedDocuments	rdf:type        owl:DatatypeProperty;	
				        rdfs:label	"hasGeneratedDocuments";
						rdfs:domain	p4-lucat:HospitalProcess;
						rdfs:range	rdfs:Literal;
						rdfs:comment "An attribute of the service reason representing the number of documents generated during the hospital process of the patient.";
						dcterms:modified "2020-07-21"^^xsd:date;
						dcterms:creator <https://www.tib.eu/en/research-development/scientific-data-management/staff/samaneh-jozashoori/>.	

p4-lucat:hasProcessCategory	rdf:type        owl:DatatypeProperty;	
				        rdfs:label	"hasProcessCategory";
						rdfs:domain	p4-lucat:HospitalProcess;
						rdfs:range	rdfs:Literal;
						rdfs:comment "An attribute of the service reason representing the type of hospital process.";
						dcterms:description "Values: it can be - cons: consultation process.- hdia-home: process which starts in 'daily hospital attendance' and finish without an ingress.- urg-hos: process which starts in 'emergencies' and finish with an ingress in hospital.- nc: no category- home_hos: process of ingress in hospital when the patient comes from home- urg_home: process of emergencies - hdia-hos: process which starts in 'daily hospital attendance' and finish with an ingress in hospital- hos-death: process that end in death for a patient that was ingressed.- urg_death: process that end in death for a patient that was in emergencies.";
						dcterms:modified "2020-07-21"^^xsd:date;
						dcterms:creator <https://www.tib.eu/en/research-development/scientific-data-management/staff/samaneh-jozashoori/>.	

p4-lucat:hasIngressDate	rdf:type        owl:DatatypeProperty;	
				        rdfs:label	"hasIngressDate";
						rdfs:domain	p4-lucat:HospitalProcess;
						rdfs:range	rdfs:Literal;
						rdfs:comment "An attribute of the service reason representing the date at which the patient was ingressed. The initiation date of the hospital process.";
						dcterms:modified "2021-03-18"^^xsd:date;
						dcterms:creator <https://www.tib.eu/en/research-development/scientific-data-management/staff/samaneh-jozashoori/>.

p4-lucat:hasDischargeDate	rdf:type        owl:DatatypeProperty;	
				        rdfs:label	"hasDischargeDate";
						rdfs:domain	p4-lucat:HospitalProcess;
						rdfs:range	rdfs:Literal;
						rdfs:comment "An attribute of the service reason representing the date at which the patient was discharged. The finishing date of the hospital process.";
						dcterms:modified "2021-03-18"^^xsd:date;
						dcterms:creator <https://www.tib.eu/en/research-development/scientific-data-management/staff/samaneh-jozashoori/>.																																																						


p4-lucat:radonRiskLevel	rdf:type owl:DatatypeProperty;	
			        rdfs:label	"radonRiskLevel";
					rdfs:domain	p4-lucat:LCPatient;
					rdfs:range	rdfs:Literal;
					rdfs:comment "";
					dcterms:modified "2020-10-29"^^xsd:date;
					dcterms:creator <https://www.tib.eu/en/research-development/scientific-data-management/staff/samaneh-jozashoori/>.

p4-lucat:diagnosisDate	rdf:type owl:DatatypeProperty;	
			        rdfs:label	"diagnosisDate";
					rdfs:domain	p4-lucat:HospitalService;
					rdfs:range	rdfs:Literal;
					rdfs:comment "";
					dcterms:modified "2021-02-05"^^xsd:date;
					dcterms:creator <https://www.tib.eu/en/research-development/scientific-data-management/staff/samaneh-jozashoori/>.

p4-lucat:hospitalized_days	rdf:type owl:DatatypeProperty;	
				        rdfs:label	"hospitalized_days";
						rdfs:domain	p4-lucat:HospitalService;
						rdfs:range	rdfs:Literal;
						rdfs:comment "";
						dcterms:modified "2021-02-05"^^xsd:date;
						dcterms:creator <https://www.tib.eu/en/research-development/scientific-data-management/staff/samaneh-jozashoori/>.

p4-lucat:days_between_firstConsultation_and_diagnosis	rdf:type owl:DatatypeProperty;	
											        rdfs:label	"days_between_firstConsultation_and_diagnosis";
													rdfs:domain	p4-lucat:HospitalService;
													rdfs:range	rdfs:Literal;
													rdfs:comment "";
													dcterms:modified "2021-02-05"^^xsd:date;
													dcterms:creator <https://www.tib.eu/en/research-development/scientific-data-management/staff/samaneh-jozashoori/>.

p4-lucat:first_consultation_date	rdf:type owl:DatatypeProperty;	
						        rdfs:label	"first_consultation_date";
								rdfs:domain	p4-lucat:HospitalService;
								rdfs:range	rdfs:Literal;
								rdfs:comment "";
								dcterms:modified "2021-02-05"^^xsd:date;
								dcterms:creator <https://www.tib.eu/en/research-development/scientific-data-management/staff/samaneh-jozashoori/>.

p4-lucat:service_percentage	rdf:type owl:DatatypeProperty;	
				        rdfs:label	"service_percentage";
						rdfs:domain	p4-lucat:HospitalService;
						rdfs:range	rdfs:Literal;
						rdfs:comment "";
						dcterms:modified "2021-02-05"^^xsd:date;
						dcterms:creator <https://www.tib.eu/en/research-development/scientific-data-management/staff/samaneh-jozashoori/>.

p4-lucat:processStartDate	rdf:type owl:DatatypeProperty;	
				        rdfs:label	"processStartDate";
						rdfs:domain	p4-lucat:HospitalService;
						rdfs:range	rdfs:Literal;
						rdfs:comment "";
						dcterms:modified "2021-02-05"^^xsd:date;
						dcterms:creator <https://www.tib.eu/en/research-development/scientific-data-management/staff/samaneh-jozashoori/>.

p4-lucat:startDate	rdf:type owl:DatatypeProperty;	
		        rdfs:label	"startDate";
				rdfs:domain	p4-lucat:HospitalService;
				rdfs:range	rdfs:Literal;
				rdfs:comment "";
				dcterms:modified "2021-02-05"^^xsd:date;
				dcterms:creator <https://www.tib.eu/en/research-development/scientific-data-management/staff/samaneh-jozashoori/>.

p4-lucat:endDate	rdf:type owl:DatatypeProperty;	
		        rdfs:label	"endDate";
				rdfs:domain	p4-lucat:HospitalService;
				rdfs:range	rdfs:Literal;
				rdfs:comment "";
				dcterms:modified "2021-02-05"^^xsd:date;
				dcterms:creator <https://www.tib.eu/en/research-development/scientific-data-management/staff/samaneh-jozashoori/>.

p4-lucat:processDescription	rdf:type owl:DatatypeProperty;	
				        rdfs:label	"processDescription";
						rdfs:domain	p4-lucat:HospitalService;
						rdfs:range	rdfs:Literal;
						rdfs:comment "";
						dcterms:modified "2021-02-05"^^xsd:date;
						dcterms:creator <https://www.tib.eu/en/research-development/scientific-data-management/staff/samaneh-jozashoori/>.

p4-lucat:service_has_scope	rdf:type owl:DatatypeProperty;	
				        rdfs:label	"service_has_scope";
						rdfs:domain	p4-lucat:HospitalService;
						rdfs:range	p4-lucat:ScopeOfService;
						rdfs:comment "";
						dcterms:modified "2021-02-05"^^xsd:date;
						dcterms:creator <https://www.tib.eu/en/research-development/scientific-data-management/staff/samaneh-jozashoori/>.

p4-lucat:service_has_type	rdf:type owl:DatatypeProperty;	
				        rdfs:label	"service_has_type";
						rdfs:domain	p4-lucat:HospitalService;
						rdfs:range	p4-lucat:TypeOfService;
						rdfs:comment "";
						dcterms:modified "2021-02-05"^^xsd:date;
						dcterms:creator <https://www.tib.eu/en/research-development/scientific-data-management/staff/samaneh-jozashoori/>.

p4-lucat:service_isRelatedTo_department	rdf:type owl:DatatypeProperty;	
							        rdfs:label	"service_isRelatedTo_department";
									rdfs:domain	p4-lucat:HospitalService;
									rdfs:range	p4-lucat:ServiceDepartment;
									rdfs:comment "";
									dcterms:modified "2021-02-05"^^xsd:date;
									dcterms:creator <https://www.tib.eu/en/research-development/scientific-data-management/staff/samaneh-jozashoori/>.

p4-lucat:is_associated_with	rdf:type owl:DatatypeProperty;	
				        rdfs:label	"is_associated_with";
						rdfs:domain	p4-lucat:HospitalService;
						rdfs:range	p4-lucat:Concept;
						rdfs:comment "";
						dcterms:modified "2021-02-05"^^xsd:date;
						dcterms:creator <https://www.tib.eu/en/research-development/scientific-data-management/staff/samaneh-jozashoori/>.


##### lc_images:

p4-lucat:bodyPartExaminedLabel     rdf:type	owl:DatatypeProperty;
							rdfs:label	"bodyPartExaminedLabel";
							rdfs:domain	p4-lucat:BodyPartExamined;
							rdfs:range	rdfs:Literal;
							rdfs:comment ".";
							dcterms:modified "2018-11-25"^^xsd:date;
							dcterms:creator <https://www.tib.eu/en/research-development/scientific-data-management/staff/maria-isabel-castellanos/>.

p4-lucat:diagnosisLabel    rdf:type	owl:DatatypeProperty;
							rdfs:label	"diagnosisLabel";
							rdfs:domain	p4-lucat:Diagnosis;
							rdfs:range	rdfs:Literal;
							rdfs:comment ".";
							dcterms:modified "2018-11-25"^^xsd:date;
							dcterms:creator <https://www.tib.eu/en/research-development/scientific-data-management/staff/maria-isabel-castellanos/>.



p4-lucat:manufacturer       rdf:type     owl:DatatypeProperty;
							rdfs:label	"manufacturer";
							rdfs:domain	p4-lucat:LCImage;
							rdfs:range	rdfs:Literal;
							rdfs:comment ".";
							dcterms:modified "2018-11-25"^^xsd:date;
							dcterms:creator <https://www.tib.eu/en/research-development/scientific-data-management/staff/maria-isabel-castellanos/>.

p4-lucat:studyDescription       rdf:type     owl:DatatypeProperty;
							rdfs:label	"studyDescription";
							rdfs:domain	p4-lucat:LCImage;
							rdfs:range	rdfs:Literal;
							rdfs:comment ".";
							dcterms:modified "2018-11-25"^^xsd:date;
							dcterms:creator <https://www.tib.eu/en/research-development/scientific-data-management/staff/maria-isabel-castellanos/>.


p4-lucat:sliceThickness       rdf:type     owl:DatatypeProperty;
							rdfs:label	"sliceThickness";
							rdfs:domain	p4-lucat:LCImage;
							rdfs:range	rdfs:Literal;
							rdfs:comment ".";
							dcterms:modified "2018-11-25"^^xsd:date;
							dcterms:creator <https://www.tib.eu/en/research-development/scientific-data-management/staff/maria-isabel-castellanos/>.

p4-lucat:protocolName       rdf:type     owl:DatatypeProperty;
							rdfs:label	"protocolName";
							rdfs:domain	p4-lucat:LCImage;
							rdfs:range	rdfs:Literal;
							rdfs:comment ".";
							dcterms:modified "2018-11-25"^^xsd:date;
							dcterms:creator <https://www.tib.eu/en/research-development/scientific-data-management/staff/maria-isabel-castellanos/>.


p4-lucat:rows       rdf:type     owl:DatatypeProperty;
							rdfs:label	"rows";
							rdfs:domain	p4-lucat:LCImage;
							rdfs:range	rdfs:Literal;
							rdfs:comment ".";
							dcterms:modified "2018-11-25"^^xsd:date;
							dcterms:creator <https://www.tib.eu/en/research-development/scientific-data-management/staff/maria-isabel-castellanos/>.

p4-lucat:columns       rdf:type     owl:DatatypeProperty;
							rdfs:label	"columns";
							rdfs:domain	p4-lucat:LCImage;
							rdfs:range	rdfs:Literal;
							rdfs:comment ".";
							dcterms:modified "2018-11-25"^^xsd:date;
							dcterms:creator <https://www.tib.eu/en/research-development/scientific-data-management/staff/maria-isabel-castellanos/>.

p4-lucat:pixelSpacingX       rdf:type     owl:DatatypeProperty;
							rdfs:label	"pixelSpacingX";
							rdfs:domain	p4-lucat:LCImage;
							rdfs:range	rdfs:Literal;
							rdfs:comment ".";
							dcterms:modified "2018-11-25"^^xsd:date;
							dcterms:creator <https://www.tib.eu/en/research-development/scientific-data-management/staff/maria-isabel-castellanos/>.

p4-lucat:pixelSpacingY      rdf:type     owl:DatatypeProperty;
							rdfs:label	"pixelSpacingY";
							rdfs:domain	p4-lucat:LCImage;
							rdfs:range	rdfs:Literal;
							rdfs:comment ".";
							dcterms:modified "2018-11-25"^^xsd:date;
							dcterms:creator <https://www.tib.eu/en/research-development/scientific-data-management/staff/maria-isabel-castellanos/>.

p4-lucat:bitsAllocated      rdf:type     owl:DatatypeProperty;
							rdfs:label	"bitsAllocated";
							rdfs:domain	p4-lucat:LCImage;
							rdfs:range	rdfs:Literal;
							rdfs:comment ".";
							dcterms:modified "2018-11-25"^^xsd:date;
							dcterms:creator <https://www.tib.eu/en/research-development/scientific-data-management/staff/maria-isabel-castellanos/>.

p4-lucat:bitsStored      rdf:type     owl:DatatypeProperty;
							rdfs:label	"bitsStored";
							rdfs:domain	p4-lucat:LCImage;
							rdfs:range	rdfs:Literal;
							rdfs:comment ".";
							dcterms:modified "2018-11-25"^^xsd:date;
							dcterms:creator <https://www.tib.eu/en/research-development/scientific-data-management/staff/maria-isabel-castellanos/>.

p4-lucat:highBit      rdf:type     owl:DatatypeProperty;
							rdfs:label	"highBit";
							rdfs:domain	p4-lucat:LCImage;
							rdfs:range	rdfs:Literal;
							rdfs:comment ".";
							dcterms:modified "2018-11-25"^^xsd:date;
							dcterms:creator <https://www.tib.eu/en/research-development/scientific-data-management/staff/maria-isabel-castellanos/>.

p4-lucat:rescaleIntercept      rdf:type     owl:DatatypeProperty;
							rdfs:label	"rescaleIntercept";
							rdfs:domain	p4-lucat:LCImage;
							rdfs:range	rdfs:Literal;
							rdfs:comment ".";
							dcterms:modified "2018-11-25"^^xsd:date;
							dcterms:creator <https://www.tib.eu/en/research-development/scientific-data-management/staff/maria-isabel-castellanos/>.

p4-lucat:rescaleSlope      rdf:type     owl:DatatypeProperty;
							rdfs:label	"rescaleSlope";
							rdfs:domain	p4-lucat:LCImage;
							rdfs:range	rdfs:Literal;
							rdfs:comment ".";
							dcterms:modified "2018-11-25"^^xsd:date;
							dcterms:creator <https://www.tib.eu/en/research-development/scientific-data-management/staff/maria-isabel-castellanos/>.

p4-lucat:huphm      rdf:type     owl:DatatypeProperty;
							rdfs:label	"huphm";
							rdfs:domain	p4-lucat:LCImage;
							rdfs:range	rdfs:Literal;
							rdfs:comment ".";
							dcterms:modified "2018-11-25"^^xsd:date;
							dcterms:creator <https://www.tib.eu/en/research-development/scientific-data-management/staff/maria-isabel-castellanos/>.


p4-lucat:lungLateralityLabel      rdf:type     owl:DatatypeProperty;
							rdfs:label	"lungLateralityLabel";
							rdfs:domain	p4-lucat:LungLaterality;
							rdfs:range	rdfs:Literal;
							rdfs:comment ".";
							dcterms:modified "2018-11-25"^^xsd:date;
							dcterms:creator <https://www.tib.eu/en/research-development/scientific-data-management/staff/maria-isabel-castellanos/>.

p4-lucat:modalityLabel      rdf:type     owl:DatatypeProperty;
							rdfs:label	"modalityLabel";
							rdfs:domain	p4-lucat:Modality;
							rdfs:range	rdfs:Literal;
							rdfs:comment ".";
							dcterms:modified "2018-11-25"^^xsd:date;
							dcterms:creator <https://www.tib.eu/en/research-development/scientific-data-management/staff/maria-isabel-castellanos/>.

p4-lucat:hasDiagnosisDate   rdf:type     owl:DatatypeProperty;
							rdfs:label	"hasDiagnosisDate";
							rdfs:domain	p4-lucat:Diagnosis;
							rdfs:range	rdfs:Literal;
							rdfs:comment ".";
							dcterms:modified "2021-03-18"^^xsd:date;
							dcterms:creator <https://www.tib.eu/en/research-development/scientific-data-management/staff/maria-isabel-castellanos/>.

p4-lucat:hasDiagnosisAge   rdf:type     owl:DatatypeProperty;
							rdfs:label	"hasDiagnosisAge";
							rdfs:domain	p4-lucat:Diagnosis;
							rdfs:range	rdfs:Literal;
							rdfs:comment ".";
							dcterms:modified "2018-11-27"^^xsd:date;
							dcterms:creator <https://www.tib.eu/en/research-development/scientific-data-management/staff/maria-isabel-castellanos/>.


p4-lucat:patientPositionLabel     rdf:type     owl:DatatypeProperty;
							rdfs:label	"patientPositionLabel";
							rdfs:domain	p4-lucat:PatientPosition;
							rdfs:range	rdfs:Literal;
							rdfs:comment ".";
							dcterms:modified "2018-11-25"^^xsd:date;
							dcterms:creator <https://www.tib.eu/en/research-development/scientific-data-management/staff/maria-isabel-castellanos/>.


p4-lucat:genderLabel_ENG        rdf:type     owl:DatatypeProperty;
							rdfs:label	"genderLabel_ENG";
							rdfs:domain	p4-lucat:Gender;
							rdfs:range	rdfs:Literal;
							rdfs:comment ".";
							dcterms:modified "2019-01-30"^^xsd:date;
							dcterms:creator <https://www.tib.eu/en/research-development/scientific-data-management/staff/samaneh-jozashoori/>.


####### lc_similarity:
p4-lucat:chemotherapyList      rdf:type     owl:DatatypeProperty;
							rdfs:label	"chemotherapyList";
							rdfs:domain	p4-lucat:LCPatient;
							rdfs:range	rdfs:Literal;
							rdfs:comment ".";
							dcterms:modified "2018-11-27"^^xsd:date;
							dcterms:creator <https://www.tib.eu/en/research-development/scientific-data-management/staff/maria-isabel-castellanos/>.


p4-lucat:immunotherapyList      rdf:type     owl:DatatypeProperty;
							rdfs:label	"immunotherapyList";
							rdfs:domain	p4-lucat:LCPatient;
							rdfs:range	rdfs:Literal;
							rdfs:comment ".";
							dcterms:modified "2018-11-27"^^xsd:date;
							dcterms:creator <https://www.tib.eu/en/research-development/scientific-data-management/staff/maria-isabel-castellanos/>.


p4-lucat:tkiList      rdf:type     owl:DatatypeProperty;
							rdfs:label	"tkiList";
							rdfs:domain	p4-lucat:LCPatient;
							rdfs:range	rdfs:Literal;
							rdfs:comment ".";
							dcterms:modified "2018-11-27"^^xsd:date;
							dcterms:creator <https://www.tib.eu/en/research-development/scientific-data-management/staff/maria-isabel-castellanos/>.

p4-lucat:comorbidityList      rdf:type     owl:DatatypeProperty;
							rdfs:label	"comorbidityList";
							rdfs:domain	p4-lucat:LCPatient;
							rdfs:range	rdfs:Literal;
							rdfs:comment ".";
							dcterms:modified "2018-11-27"^^xsd:date;
							dcterms:creator <https://www.tib.eu/en/research-development/scientific-data-management/staff/maria-isabel-castellanos/>.

p4-lucat:drugGroupList      rdf:type     owl:DatatypeProperty;
							rdfs:label	"drugGroupList";
							rdfs:domain	p4-lucat:LCPatient;
							rdfs:range	rdfs:Literal;
							rdfs:comment ".";
							dcterms:modified "2018-11-27"^^xsd:date;
							dcterms:creator <https://www.tib.eu/en/research-development/scientific-data-management/staff/maria-isabel-castellanos/>.

p4-lucat:biopsyList      rdf:type     owl:DatatypeProperty;
							rdfs:label	"biopsyList";
							rdfs:domain	p4-lucat:LCPatient;
							rdfs:range	rdfs:Literal;
							rdfs:comment ".";
							dcterms:modified "2018-11-27"^^xsd:date;
							dcterms:creator <https://www.tib.eu/en/research-development/scientific-data-management/staff/maria-isabel-castellanos/>.

p4-lucat:ecogList      rdf:type     owl:DatatypeProperty;
							rdfs:label	"ecogList";
							rdfs:domain	p4-lucat:LCPatient;
							rdfs:range	rdfs:Literal;
							rdfs:comment ".";
							dcterms:modified "2018-11-27"^^xsd:date;
							dcterms:creator <https://www.tib.eu/en/research-development/scientific-data-management/staff/maria-isabel-castellanos/>.

p4-lucat:stageList      rdf:type     owl:DatatypeProperty;
							rdfs:label	"stageList";
							rdfs:domain	p4-lucat:LCPatient;
							rdfs:range	rdfs:Literal;
							rdfs:comment ".";
							dcterms:modified "2018-11-27"^^xsd:date;
							dcterms:creator <https://www.tib.eu/en/research-development/scientific-data-management/staff/maria-isabel-castellanos/>.

p4-lucat:familialAntecedentList      rdf:type     owl:DatatypeProperty;
							rdfs:label	"familialAntecedentList";
							rdfs:domain	p4-lucat:LCPatient;
							rdfs:range	rdfs:Literal;
							rdfs:comment ".";
							dcterms:modified "2018-11-27"^^xsd:date;
							dcterms:creator <https://www.tib.eu/en/research-development/scientific-data-management/staff/maria-isabel-castellanos/>.

p4-lucat:nonOncologicalTreatmentList      rdf:type     owl:DatatypeProperty;
							rdfs:label	"nonOncologicalTreatmentList";
							rdfs:domain	p4-lucat:LCPatient;
							rdfs:range	rdfs:Literal;
							rdfs:comment ".";
							dcterms:modified "2018-11-27"^^xsd:date;
							dcterms:creator <https://www.tib.eu/en/research-development/scientific-data-management/staff/maria-isabel-castellanos/>.


p4-lucat:similarityValue     rdf:type     owl:DatatypeProperty;
							rdfs:label	"similarityValue";
							rdfs:domain	p4-lucat:LCPatient;
							rdfs:range	rdfs:Literal;
							rdfs:comment ".";
							dcterms:modified "2018-11-27"^^xsd:date;
							dcterms:creator <https://www.tib.eu/en/research-development/scientific-data-management/staff/maria-isabel-castellanos/>.
